<?xml version="1.0"?>
<rdf:RDF xmlns="http://purl.unep.org/sdg/imports/envo_import.owl#"
     xml:base="http://purl.unep.org/sdg/imports/envo_import.owl"
     xmlns:rdf="http://www.w3.org/1999/02/22-rdf-syntax-ns#"
     xmlns:owl="http://www.w3.org/2002/07/owl#"
     xmlns:oboInOwl="http://www.geneontology.org/formats/oboInOwl#"
     xmlns:xsd="http://www.w3.org/2001/XMLSchema#"
     xmlns:rdfs="http://www.w3.org/2000/01/rdf-schema#"
     xmlns:obo="http://purl.obolibrary.org/obo/">
    <owl:Ontology rdf:about="http://purl.unep.org/sdg/imports/envo_import.owl"/>
    


    <!-- 
    ///////////////////////////////////////////////////////////////////////////////////////
    //
    // Annotation properties
    //
    ///////////////////////////////////////////////////////////////////////////////////////
     -->

    


    <!-- http://purl.obolibrary.org/obo/IAO_0000115 -->

    <owl:AnnotationProperty rdf:about="http://purl.obolibrary.org/obo/IAO_0000115"/>
    


    <!-- http://www.geneontology.org/formats/oboInOwl#hasBroadSynonym -->

    <owl:AnnotationProperty rdf:about="http://www.geneontology.org/formats/oboInOwl#hasBroadSynonym"/>
    


    <!-- http://www.geneontology.org/formats/oboInOwl#hasExactSynonym -->

    <owl:AnnotationProperty rdf:about="http://www.geneontology.org/formats/oboInOwl#hasExactSynonym"/>
    


    <!-- http://www.geneontology.org/formats/oboInOwl#hasNarrowSynonym -->

    <owl:AnnotationProperty rdf:about="http://www.geneontology.org/formats/oboInOwl#hasNarrowSynonym"/>
    


    <!-- http://www.geneontology.org/formats/oboInOwl#hasRelatedSynonym -->

    <owl:AnnotationProperty rdf:about="http://www.geneontology.org/formats/oboInOwl#hasRelatedSynonym"/>
    


    <!-- 
    ///////////////////////////////////////////////////////////////////////////////////////
    //
    // Classes
    //
    ///////////////////////////////////////////////////////////////////////////////////////
     -->

    


    <!-- http://purl.obolibrary.org/obo/BFO_0000002 -->

    <owl:Class rdf:about="http://purl.obolibrary.org/obo/BFO_0000002">
        <rdfs:label xml:lang="en">continuant</rdfs:label>
        <obo:IAO_0000115 xml:lang="en">An entity that exists in full at any time in which it exists at all, persists through time while maintaining its identity and has no temporal parts.</obo:IAO_0000115>
    </owl:Class>
    


    <!-- http://purl.obolibrary.org/obo/BFO_0000003 -->

    <owl:Class rdf:about="http://purl.obolibrary.org/obo/BFO_0000003">
        <rdfs:label xml:lang="en">occurrent</rdfs:label>
        <obo:IAO_0000115 xml:lang="en">An entity that has temporal parts and that happens, unfolds or develops through time.</obo:IAO_0000115>
    </owl:Class>
    


    <!-- http://purl.obolibrary.org/obo/BFO_0000004 -->

    <owl:Class rdf:about="http://purl.obolibrary.org/obo/BFO_0000004">
        <rdfs:label xml:lang="en">independent continuant</rdfs:label>
        <rdfs:subClassOf rdf:resource="http://purl.obolibrary.org/obo/BFO_0000002"/>
        <obo:IAO_0000115 xml:lang="en">A continuant that is a bearer of quality and realizable entity entities, in which other entities inhere and which itself cannot inhere in anything.</obo:IAO_0000115>
    </owl:Class>
    


    <!-- http://purl.obolibrary.org/obo/BFO_0000015 -->

    <owl:Class rdf:about="http://purl.obolibrary.org/obo/BFO_0000015">
        <rdfs:label xml:lang="en">process</rdfs:label>
        <rdfs:subClassOf rdf:resource="http://purl.obolibrary.org/obo/BFO_0000003"/>
        <obo:IAO_0000115 xml:lang="en">An occurrent that has temporal proper parts and for some time t, p s-depends_on some material entity at t.</obo:IAO_0000115>
    </owl:Class>
    


    <!-- http://purl.obolibrary.org/obo/BFO_0000017 -->

    <owl:Class rdf:about="http://purl.obolibrary.org/obo/BFO_0000017">
        <rdfs:label xml:lang="en">realizable entity</rdfs:label>
        <rdfs:subClassOf rdf:resource="http://purl.obolibrary.org/obo/BFO_0000020"/>
        <obo:IAO_0000115 xml:lang="en">A specifically dependent continuant  that inheres in continuant  entities and are not exhibited in full at every time in which it inheres in an entity or group of entities. The exhibition or actualization of a realizable entity is a particular manifestation, functioning or process that occurs under certain circumstances.</obo:IAO_0000115>
    </owl:Class>
    


    <!-- http://purl.obolibrary.org/obo/BFO_0000020 -->

    <owl:Class rdf:about="http://purl.obolibrary.org/obo/BFO_0000020">
        <rdfs:label xml:lang="en">specifically dependent continuant</rdfs:label>
        <rdfs:subClassOf rdf:resource="http://purl.obolibrary.org/obo/BFO_0000002"/>
        <obo:IAO_0000115 xml:lang="en">A continuant that inheres in or is borne by other entities. Every instance of A requires some specific instance of B which must always be the same.</obo:IAO_0000115>
    </owl:Class>
    


    <!-- http://purl.obolibrary.org/obo/BFO_0000023 -->

    <owl:Class rdf:about="http://purl.obolibrary.org/obo/BFO_0000023">
        <rdfs:label xml:lang="en">role</rdfs:label>
        <rdfs:subClassOf rdf:resource="http://purl.obolibrary.org/obo/BFO_0000017"/>
        <obo:IAO_0000115 xml:lang="en">A realizable entity  the manifestation of which brings about some result or end that is not essential to a continuant  in virtue of the kind of thing that it is but that can be served or participated in by that kind of continuant  in some kinds of natural, social or institutional contexts.</obo:IAO_0000115>
    </owl:Class>
    


    <!-- http://purl.obolibrary.org/obo/BFO_0000040 -->

    <owl:Class rdf:about="http://purl.obolibrary.org/obo/BFO_0000040">
        <rdfs:label xml:lang="en">material entity</rdfs:label>
        <rdfs:subClassOf rdf:resource="http://purl.obolibrary.org/obo/BFO_0000004"/>
        <obo:IAO_0000115 xml:lang="en">An independent continuant that is spatially extended whose identity is independent of that of other entities and can be maintained through time.</obo:IAO_0000115>
    </owl:Class>
    


    <!-- http://purl.obolibrary.org/obo/ENVO_00000000 -->

    <owl:Class rdf:about="http://purl.obolibrary.org/obo/ENVO_00000000">
        <rdfs:label rdf:datatype="http://www.w3.org/2001/XMLSchema#string">geographic feature</rdfs:label>
        <rdfs:subClassOf rdf:resource="http://purl.obolibrary.org/obo/ENVO_00002297"/>
        <oboInOwl:hasExactSynonym rdf:datatype="http://www.w3.org/2001/XMLSchema#string">macroscopic spatial feature</oboInOwl:hasExactSynonym>
    </owl:Class>
    


    <!-- http://purl.obolibrary.org/obo/ENVO_00000002 -->

    <owl:Class rdf:about="http://purl.obolibrary.org/obo/ENVO_00000002">
        <rdfs:label rdf:datatype="http://www.w3.org/2001/XMLSchema#string">anthropogenic geographic feature</rdfs:label>
        <rdfs:subClassOf rdf:resource="http://purl.obolibrary.org/obo/ENVO_00000000"/>
        <obo:IAO_0000115 rdf:datatype="http://www.w3.org/2001/XMLSchema#string">An anthropogenic geographic feature is a geographic feature
resulting from the influence of human beings on nature.</obo:IAO_0000115>
        <oboInOwl:hasRelatedSynonym rdf:datatype="http://www.w3.org/2001/XMLSchema#string">man-made feature</oboInOwl:hasRelatedSynonym>
        <oboInOwl:hasRelatedSynonym rdf:datatype="http://www.w3.org/2001/XMLSchema#string">manmade feature</oboInOwl:hasRelatedSynonym>
    </owl:Class>
    


    <!-- http://purl.obolibrary.org/obo/ENVO_00000015 -->

    <owl:Class rdf:about="http://purl.obolibrary.org/obo/ENVO_00000015">
        <rdfs:label rdf:datatype="http://www.w3.org/2001/XMLSchema#string">ocean</rdfs:label>
        <rdfs:subClassOf rdf:resource="http://purl.obolibrary.org/obo/ENVO_00001999"/>
        <obo:IAO_0000115 rdf:datatype="http://www.w3.org/2001/XMLSchema#string">Continuous saline-water bodies that surround the continents and fill the Earth&apos;s great depressions.</obo:IAO_0000115>
        <oboInOwl:hasExactSynonym rdf:datatype="http://www.w3.org/2001/XMLSchema#string">Ocean</oboInOwl:hasExactSynonym>
        <oboInOwl:hasExactSynonym rdf:datatype="http://www.w3.org/2001/XMLSchema#string">ocean</oboInOwl:hasExactSynonym>
        <oboInOwl:hasRelatedSynonym rdf:datatype="http://www.w3.org/2001/XMLSchema#string">ocean region</oboInOwl:hasRelatedSynonym>
        <oboInOwl:hasRelatedSynonym rdf:datatype="http://www.w3.org/2001/XMLSchema#string">sea</oboInOwl:hasRelatedSynonym>
    </owl:Class>
    


    <!-- http://purl.obolibrary.org/obo/ENVO_00000016 -->

    <owl:Class rdf:about="http://purl.obolibrary.org/obo/ENVO_00000016">
        <rdfs:label rdf:datatype="http://www.w3.org/2001/XMLSchema#string">sea</rdfs:label>
        <rdfs:subClassOf rdf:resource="http://purl.obolibrary.org/obo/ENVO_00001999"/>
        <obo:IAO_0000115 rdf:datatype="http://www.w3.org/2001/XMLSchema#string">A large expanse of saline water usually connected with an ocean.</obo:IAO_0000115>
        <oboInOwl:hasExactSynonym rdf:datatype="http://www.w3.org/2001/XMLSchema#string">Sea</oboInOwl:hasExactSynonym>
        <oboInOwl:hasNarrowSynonym rdf:datatype="http://www.w3.org/2001/XMLSchema#string">channel</oboInOwl:hasNarrowSynonym>
        <oboInOwl:hasNarrowSynonym rdf:datatype="http://www.w3.org/2001/XMLSchema#string">closed sea</oboInOwl:hasNarrowSynonym>
        <oboInOwl:hasNarrowSynonym rdf:datatype="http://www.w3.org/2001/XMLSchema#string">marginal sea</oboInOwl:hasNarrowSynonym>
        <oboInOwl:hasNarrowSynonym rdf:datatype="http://www.w3.org/2001/XMLSchema#string">open sea</oboInOwl:hasNarrowSynonym>
        <oboInOwl:hasNarrowSynonym rdf:datatype="http://www.w3.org/2001/XMLSchema#string">open sound</oboInOwl:hasNarrowSynonym>
        <oboInOwl:hasNarrowSynonym rdf:datatype="http://www.w3.org/2001/XMLSchema#string">open water</oboInOwl:hasNarrowSynonym>
        <oboInOwl:hasExactSynonym rdf:datatype="http://www.w3.org/2001/XMLSchema#string">sea</oboInOwl:hasExactSynonym>
    </owl:Class>
    


    <!-- http://purl.obolibrary.org/obo/ENVO_00000020 -->

    <owl:Class rdf:about="http://purl.obolibrary.org/obo/ENVO_00000020">
        <rdfs:label rdf:datatype="http://www.w3.org/2001/XMLSchema#string">lake</rdfs:label>
        <rdfs:subClassOf rdf:resource="http://purl.obolibrary.org/obo/ENVO_01000617"/>
        <obo:IAO_0000115 rdf:datatype="http://www.w3.org/2001/XMLSchema#string">A body of water or other liquid of considerable size contained on a body of land.</obo:IAO_0000115>
        <oboInOwl:hasExactSynonym rdf:datatype="http://www.w3.org/2001/XMLSchema#string">LAKE</oboInOwl:hasExactSynonym>
        <oboInOwl:hasExactSynonym rdf:datatype="http://www.w3.org/2001/XMLSchema#string">Lake</oboInOwl:hasExactSynonym>
        <oboInOwl:hasRelatedSynonym rdf:datatype="http://www.w3.org/2001/XMLSchema#string">broad</oboInOwl:hasRelatedSynonym>
        <oboInOwl:hasNarrowSynonym rdf:datatype="http://www.w3.org/2001/XMLSchema#string">catch basin</oboInOwl:hasNarrowSynonym>
        <oboInOwl:hasExactSynonym rdf:datatype="http://www.w3.org/2001/XMLSchema#string">lake</oboInOwl:hasExactSynonym>
        <oboInOwl:hasExactSynonym rdf:datatype="http://www.w3.org/2001/XMLSchema#string">lakes</oboInOwl:hasExactSynonym>
        <oboInOwl:hasRelatedSynonym rdf:datatype="http://www.w3.org/2001/XMLSchema#string">llyn</oboInOwl:hasRelatedSynonym>
        <oboInOwl:hasRelatedSynonym rdf:datatype="http://www.w3.org/2001/XMLSchema#string">loch</oboInOwl:hasRelatedSynonym>
        <oboInOwl:hasRelatedSynonym rdf:datatype="http://www.w3.org/2001/XMLSchema#string">lochan</oboInOwl:hasRelatedSynonym>
        <oboInOwl:hasRelatedSynonym rdf:datatype="http://www.w3.org/2001/XMLSchema#string">lough</oboInOwl:hasRelatedSynonym>
        <oboInOwl:hasRelatedSynonym rdf:datatype="http://www.w3.org/2001/XMLSchema#string">mere</oboInOwl:hasRelatedSynonym>
        <oboInOwl:hasRelatedSynonym rdf:datatype="http://www.w3.org/2001/XMLSchema#string">mortlake</oboInOwl:hasRelatedSynonym>
        <oboInOwl:hasNarrowSynonym rdf:datatype="http://www.w3.org/2001/XMLSchema#string">open water</oboInOwl:hasNarrowSynonym>
        <oboInOwl:hasRelatedSynonym rdf:datatype="http://www.w3.org/2001/XMLSchema#string">pasteuer lake</oboInOwl:hasRelatedSynonym>
        <oboInOwl:hasNarrowSynonym rdf:datatype="http://www.w3.org/2001/XMLSchema#string">tarn</oboInOwl:hasNarrowSynonym>
    </owl:Class>
    


    <!-- http://purl.obolibrary.org/obo/ENVO_00000022 -->

    <owl:Class rdf:about="http://purl.obolibrary.org/obo/ENVO_00000022">
        <rdfs:label rdf:datatype="http://www.w3.org/2001/XMLSchema#string">river</rdfs:label>
        <rdfs:subClassOf rdf:resource="http://purl.obolibrary.org/obo/ENVO_00000023"/>
        <obo:IAO_0000115 rdf:datatype="http://www.w3.org/2001/XMLSchema#string">Natural freshwater surface streams of considerable volume and a permanent or seasonal flow, moving in a definite channel toward a sea, lake, or another river; any large streams, or ones larger than brooks or creeks, such as the trunk stream and larger branches of a drainage system.</obo:IAO_0000115>
        <oboInOwl:hasExactSynonym rdf:datatype="http://www.w3.org/2001/XMLSchema#string">River</oboInOwl:hasExactSynonym>
        <oboInOwl:hasNarrowSynonym rdf:datatype="http://www.w3.org/2001/XMLSchema#string">braided river</oboInOwl:hasNarrowSynonym>
        <oboInOwl:hasExactSynonym rdf:datatype="http://www.w3.org/2001/XMLSchema#string">rio</oboInOwl:hasExactSynonym>
        <oboInOwl:hasBroadSynonym rdf:datatype="http://www.w3.org/2001/XMLSchema#string">watercourse</oboInOwl:hasBroadSynonym>
    </owl:Class>
    


    <!-- http://purl.obolibrary.org/obo/ENVO_00000023 -->

    <owl:Class rdf:about="http://purl.obolibrary.org/obo/ENVO_00000023">
        <rdfs:label rdf:datatype="http://www.w3.org/2001/XMLSchema#string">stream</rdfs:label>
        <rdfs:subClassOf rdf:resource="http://purl.obolibrary.org/obo/ENVO_00000029"/>
        <oboInOwl:hasRelatedSynonym rdf:datatype="http://www.w3.org/2001/XMLSchema#string">Creek</oboInOwl:hasRelatedSynonym>
        <obo:IAO_0000115 rdf:datatype="http://www.w3.org/2001/XMLSchema#string">Linear body of water flowing on the Earth&apos;s surface.</obo:IAO_0000115>
        <oboInOwl:hasExactSynonym rdf:datatype="http://www.w3.org/2001/XMLSchema#string">Stream</oboInOwl:hasExactSynonym>
        <oboInOwl:hasRelatedSynonym rdf:datatype="http://www.w3.org/2001/XMLSchema#string">beck</oboInOwl:hasRelatedSynonym>
        <oboInOwl:hasNarrowSynonym rdf:datatype="http://www.w3.org/2001/XMLSchema#string">braided stream</oboInOwl:hasNarrowSynonym>
        <oboInOwl:hasRelatedSynonym rdf:datatype="http://www.w3.org/2001/XMLSchema#string">brook</oboInOwl:hasRelatedSynonym>
        <oboInOwl:hasRelatedSynonym rdf:datatype="http://www.w3.org/2001/XMLSchema#string">burn (hydrographic)</oboInOwl:hasRelatedSynonym>
        <oboInOwl:hasRelatedSynonym rdf:datatype="http://www.w3.org/2001/XMLSchema#string">creek</oboInOwl:hasRelatedSynonym>
        <oboInOwl:hasNarrowSynonym rdf:datatype="http://www.w3.org/2001/XMLSchema#string">fork (hydrographic</oboInOwl:hasNarrowSynonym>
        <oboInOwl:hasNarrowSynonym rdf:datatype="http://www.w3.org/2001/XMLSchema#string">glacial stream</oboInOwl:hasNarrowSynonym>
        <oboInOwl:hasNarrowSynonym rdf:datatype="http://www.w3.org/2001/XMLSchema#string">lode</oboInOwl:hasNarrowSynonym>
        <oboInOwl:hasNarrowSynonym rdf:datatype="http://www.w3.org/2001/XMLSchema#string">millstream</oboInOwl:hasNarrowSynonym>
        <oboInOwl:hasRelatedSynonym rdf:datatype="http://www.w3.org/2001/XMLSchema#string">rivulet</oboInOwl:hasRelatedSynonym>
        <oboInOwl:hasExactSynonym rdf:datatype="http://www.w3.org/2001/XMLSchema#string">stream</oboInOwl:hasExactSynonym>
        <oboInOwl:hasNarrowSynonym rdf:datatype="http://www.w3.org/2001/XMLSchema#string">stream bend</oboInOwl:hasNarrowSynonym>
        <oboInOwl:hasExactSynonym rdf:datatype="http://www.w3.org/2001/XMLSchema#string">streams</oboInOwl:hasExactSynonym>
        <oboInOwl:hasBroadSynonym rdf:datatype="http://www.w3.org/2001/XMLSchema#string">watercourse</oboInOwl:hasBroadSynonym>
    </owl:Class>
    


    <!-- http://purl.obolibrary.org/obo/ENVO_00000029 -->

    <owl:Class rdf:about="http://purl.obolibrary.org/obo/ENVO_00000029">
        <rdfs:label rdf:datatype="http://www.w3.org/2001/XMLSchema#string">watercourse</rdfs:label>
        <rdfs:subClassOf rdf:resource="http://purl.obolibrary.org/obo/ENVO_01000618"/>
        <obo:IAO_0000115 rdf:datatype="http://www.w3.org/2001/XMLSchema#string">A flowing body of water.</obo:IAO_0000115>
        <oboInOwl:hasExactSynonym rdf:datatype="http://www.w3.org/2001/XMLSchema#string">WATERCOURSE</oboInOwl:hasExactSynonym>
        <oboInOwl:hasRelatedSynonym rdf:datatype="http://www.w3.org/2001/XMLSchema#string">awawa</oboInOwl:hasRelatedSynonym>
        <oboInOwl:hasRelatedSynonym rdf:datatype="http://www.w3.org/2001/XMLSchema#string">barranca</oboInOwl:hasRelatedSynonym>
        <oboInOwl:hasRelatedSynonym rdf:datatype="http://www.w3.org/2001/XMLSchema#string">beck</oboInOwl:hasRelatedSynonym>
        <oboInOwl:hasRelatedSynonym rdf:datatype="http://www.w3.org/2001/XMLSchema#string">branch</oboInOwl:hasRelatedSynonym>
        <oboInOwl:hasRelatedSynonym rdf:datatype="http://www.w3.org/2001/XMLSchema#string">brook</oboInOwl:hasRelatedSynonym>
        <oboInOwl:hasRelatedSynonym rdf:datatype="http://www.w3.org/2001/XMLSchema#string">course</oboInOwl:hasRelatedSynonym>
        <oboInOwl:hasNarrowSynonym rdf:datatype="http://www.w3.org/2001/XMLSchema#string">culvert</oboInOwl:hasNarrowSynonym>
        <oboInOwl:hasRelatedSynonym rdf:datatype="http://www.w3.org/2001/XMLSchema#string">draw</oboInOwl:hasRelatedSynonym>
        <oboInOwl:hasNarrowSynonym rdf:datatype="http://www.w3.org/2001/XMLSchema#string">dredged channel</oboInOwl:hasNarrowSynonym>
        <oboInOwl:hasNarrowSynonym rdf:datatype="http://www.w3.org/2001/XMLSchema#string">fork</oboInOwl:hasNarrowSynonym>
        <oboInOwl:hasNarrowSynonym rdf:datatype="http://www.w3.org/2001/XMLSchema#string">gulch</oboInOwl:hasNarrowSynonym>
        <oboInOwl:hasNarrowSynonym rdf:datatype="http://www.w3.org/2001/XMLSchema#string">gully</oboInOwl:hasNarrowSynonym>
        <oboInOwl:hasNarrowSynonym rdf:datatype="http://www.w3.org/2001/XMLSchema#string">gut</oboInOwl:hasNarrowSynonym>
        <oboInOwl:hasNarrowSynonym rdf:datatype="http://www.w3.org/2001/XMLSchema#string">gutter</oboInOwl:hasNarrowSynonym>
        <oboInOwl:hasNarrowSynonym rdf:datatype="http://www.w3.org/2001/XMLSchema#string">kill</oboInOwl:hasNarrowSynonym>
        <oboInOwl:hasNarrowSynonym rdf:datatype="http://www.w3.org/2001/XMLSchema#string">lode</oboInOwl:hasNarrowSynonym>
        <oboInOwl:hasRelatedSynonym rdf:datatype="http://www.w3.org/2001/XMLSchema#string">moat</oboInOwl:hasRelatedSynonym>
        <oboInOwl:hasRelatedSynonym rdf:datatype="http://www.w3.org/2001/XMLSchema#string">narrows</oboInOwl:hasRelatedSynonym>
        <oboInOwl:hasNarrowSynonym rdf:datatype="http://www.w3.org/2001/XMLSchema#string">narrows</oboInOwl:hasNarrowSynonym>
        <oboInOwl:hasRelatedSynonym rdf:datatype="http://www.w3.org/2001/XMLSchema#string">narrows (hydrographic)</oboInOwl:hasRelatedSynonym>
        <oboInOwl:hasNarrowSynonym rdf:datatype="http://www.w3.org/2001/XMLSchema#string">overflow channel</oboInOwl:hasNarrowSynonym>
        <oboInOwl:hasNarrowSynonym rdf:datatype="http://www.w3.org/2001/XMLSchema#string">passage</oboInOwl:hasNarrowSynonym>
        <oboInOwl:hasNarrowSynonym rdf:datatype="http://www.w3.org/2001/XMLSchema#string">pup</oboInOwl:hasNarrowSynonym>
        <oboInOwl:hasNarrowSynonym rdf:datatype="http://www.w3.org/2001/XMLSchema#string">race</oboInOwl:hasNarrowSynonym>
        <oboInOwl:hasNarrowSynonym rdf:datatype="http://www.w3.org/2001/XMLSchema#string">ravine</oboInOwl:hasNarrowSynonym>
        <oboInOwl:hasNarrowSynonym rdf:datatype="http://www.w3.org/2001/XMLSchema#string">reach</oboInOwl:hasNarrowSynonym>
        <oboInOwl:hasNarrowSynonym rdf:datatype="http://www.w3.org/2001/XMLSchema#string">rill</oboInOwl:hasNarrowSynonym>
        <oboInOwl:hasNarrowSynonym rdf:datatype="http://www.w3.org/2001/XMLSchema#string">rio</oboInOwl:hasNarrowSynonym>
        <oboInOwl:hasNarrowSynonym rdf:datatype="http://www.w3.org/2001/XMLSchema#string">rivulet</oboInOwl:hasNarrowSynonym>
        <oboInOwl:hasNarrowSynonym rdf:datatype="http://www.w3.org/2001/XMLSchema#string">run</oboInOwl:hasNarrowSynonym>
        <oboInOwl:hasNarrowSynonym rdf:datatype="http://www.w3.org/2001/XMLSchema#string">runnel</oboInOwl:hasNarrowSynonym>
        <oboInOwl:hasNarrowSynonym rdf:datatype="http://www.w3.org/2001/XMLSchema#string">seachannel</oboInOwl:hasNarrowSynonym>
        <oboInOwl:hasNarrowSynonym rdf:datatype="http://www.w3.org/2001/XMLSchema#string">seaway</oboInOwl:hasNarrowSynonym>
        <oboInOwl:hasNarrowSynonym rdf:datatype="http://www.w3.org/2001/XMLSchema#string">spillway</oboInOwl:hasNarrowSynonym>
        <oboInOwl:hasNarrowSynonym rdf:datatype="http://www.w3.org/2001/XMLSchema#string">stream</oboInOwl:hasNarrowSynonym>
        <oboInOwl:hasNarrowSynonym rdf:datatype="http://www.w3.org/2001/XMLSchema#string">tideway</oboInOwl:hasNarrowSynonym>
        <oboInOwl:hasNarrowSynonym rdf:datatype="http://www.w3.org/2001/XMLSchema#string">wash</oboInOwl:hasNarrowSynonym>
        <oboInOwl:hasNarrowSynonym rdf:datatype="http://www.w3.org/2001/XMLSchema#string">water gap</oboInOwl:hasNarrowSynonym>
        <oboInOwl:hasExactSynonym rdf:datatype="http://www.w3.org/2001/XMLSchema#string">watercourse</oboInOwl:hasExactSynonym>
        <oboInOwl:hasRelatedSynonym rdf:datatype="http://www.w3.org/2001/XMLSchema#string">waterway</oboInOwl:hasRelatedSynonym>
    </owl:Class>
    


    <!-- http://purl.obolibrary.org/obo/ENVO_00000062 -->

    <owl:Class rdf:about="http://purl.obolibrary.org/obo/ENVO_00000062">
        <rdfs:label rdf:datatype="http://www.w3.org/2001/XMLSchema#string">populated place</rdfs:label>
        <rdfs:subClassOf rdf:resource="http://purl.obolibrary.org/obo/ENVO_00000070"/>
        <obo:IAO_0000115 rdf:datatype="http://www.w3.org/2001/XMLSchema#string">Place or area with clustered or scattered buildings and a permanent human population.</obo:IAO_0000115>
        <oboInOwl:hasExactSynonym rdf:datatype="http://www.w3.org/2001/XMLSchema#string">inhabited place</oboInOwl:hasExactSynonym>
        <oboInOwl:hasRelatedSynonym rdf:datatype="http://www.w3.org/2001/XMLSchema#string">inhabited region</oboInOwl:hasRelatedSynonym>
        <oboInOwl:hasBroadSynonym rdf:datatype="http://www.w3.org/2001/XMLSchema#string">place</oboInOwl:hasBroadSynonym>
        <oboInOwl:hasRelatedSynonym rdf:datatype="http://www.w3.org/2001/XMLSchema#string">populated locality</oboInOwl:hasRelatedSynonym>
        <oboInOwl:hasExactSynonym rdf:datatype="http://www.w3.org/2001/XMLSchema#string">populated place</oboInOwl:hasExactSynonym>
        <oboInOwl:hasExactSynonym rdf:datatype="http://www.w3.org/2001/XMLSchema#string">populated places</oboInOwl:hasExactSynonym>
        <oboInOwl:hasExactSynonym rdf:datatype="http://www.w3.org/2001/XMLSchema#string">settlement</oboInOwl:hasExactSynonym>
    </owl:Class>
    


    <!-- http://purl.obolibrary.org/obo/ENVO_00000063 -->

    <owl:Class rdf:about="http://purl.obolibrary.org/obo/ENVO_00000063">
        <rdfs:label rdf:datatype="http://www.w3.org/2001/XMLSchema#string">water body</rdfs:label>
        <rdfs:subClassOf rdf:resource="http://purl.obolibrary.org/obo/ENVO_00000000"/>
        <obo:IAO_0000115 rdf:datatype="http://www.w3.org/2001/XMLSchema#string">An accumulation of water of varying size.</obo:IAO_0000115>
        <oboInOwl:hasExactSynonym rdf:datatype="http://www.w3.org/2001/XMLSchema#string">aquatic feature</oboInOwl:hasExactSynonym>
        <oboInOwl:hasExactSynonym rdf:datatype="http://www.w3.org/2001/XMLSchema#string">bodies of water</oboInOwl:hasExactSynonym>
        <oboInOwl:hasExactSynonym rdf:datatype="http://www.w3.org/2001/XMLSchema#string">body of water</oboInOwl:hasExactSynonym>
        <oboInOwl:hasBroadSynonym rdf:datatype="http://www.w3.org/2001/XMLSchema#string">hydrographic feature</oboInOwl:hasBroadSynonym>
        <oboInOwl:hasExactSynonym rdf:datatype="http://www.w3.org/2001/XMLSchema#string">waterbody</oboInOwl:hasExactSynonym>
    </owl:Class>
    


    <!-- http://purl.obolibrary.org/obo/ENVO_00000070 -->

    <owl:Class rdf:about="http://purl.obolibrary.org/obo/ENVO_00000070">
        <rdfs:label rdf:datatype="http://www.w3.org/2001/XMLSchema#string">constructed feature</rdfs:label>
        <rdfs:subClassOf rdf:resource="http://purl.obolibrary.org/obo/ENVO_00000002"/>
        <obo:IAO_0000115 rdf:datatype="http://www.w3.org/2001/XMLSchema#string">A feature that has been constructed by deliberate human effort.</obo:IAO_0000115>
    </owl:Class>
    


    <!-- http://purl.obolibrary.org/obo/ENVO_00000358 -->

    <owl:Class rdf:about="http://purl.obolibrary.org/obo/ENVO_00000358">
        <rdfs:label rdf:datatype="http://www.w3.org/2001/XMLSchema#string">protected area</rdfs:label>
        <rdfs:subClassOf rdf:resource="http://purl.obolibrary.org/obo/ENVO_00000562"/>
        <obo:IAO_0000115 rdf:datatype="http://www.w3.org/2001/XMLSchema#string">An area of land and/or a body of water especially dedicated to the protection and maintenance of biological diversity, and of natural and associated cultural resources, and managed through legal or other effective means.</obo:IAO_0000115>
    </owl:Class>
    


    <!-- http://purl.obolibrary.org/obo/ENVO_00000428 -->

    <owl:Class rdf:about="http://purl.obolibrary.org/obo/ENVO_00000428">
        <rdfs:label>biome</rdfs:label>
        <rdfs:subClassOf rdf:resource="http://purl.obolibrary.org/obo/ENVO_01000254"/>
        <obo:IAO_0000115 rdf:datatype="http://www.w3.org/2001/XMLSchema#string">A biome is an environmental system to which resident ecological communities have evolved adaptations.</obo:IAO_0000115>
        <oboInOwl:hasRelatedSynonym rdf:datatype="http://www.w3.org/2001/XMLSchema#string">EcosytemType</oboInOwl:hasRelatedSynonym>
        <oboInOwl:hasRelatedSynonym rdf:datatype="http://www.w3.org/2001/XMLSchema#string">ecosystem</oboInOwl:hasRelatedSynonym>
        <oboInOwl:hasExactSynonym rdf:datatype="http://www.w3.org/2001/XMLSchema#string">major habitat type</oboInOwl:hasExactSynonym>
    </owl:Class>
    


    <!-- http://purl.obolibrary.org/obo/ENVO_00000446 -->

    <owl:Class rdf:about="http://purl.obolibrary.org/obo/ENVO_00000446">
        <rdfs:label rdf:datatype="http://www.w3.org/2001/XMLSchema#string">terrestrial biome</rdfs:label>
        <rdfs:subClassOf rdf:resource="http://purl.obolibrary.org/obo/ENVO_00000428"/>
        <obo:IAO_0000115 rdf:datatype="http://www.w3.org/2001/XMLSchema#string">A biome that applies to the terrestrial realm.</obo:IAO_0000115>
        <oboInOwl:hasRelatedSynonym rdf:datatype="http://www.w3.org/2001/XMLSchema#string">terrestrial realm</oboInOwl:hasRelatedSynonym>
    </owl:Class>
    


    <!-- http://purl.obolibrary.org/obo/ENVO_00000562 -->

    <owl:Class rdf:about="http://purl.obolibrary.org/obo/ENVO_00000562">
        <rdfs:label rdf:datatype="http://www.w3.org/2001/XMLSchema#string">park</rdfs:label>
        <rdfs:subClassOf rdf:resource="http://purl.obolibrary.org/obo/ENVO_00000002"/>
        <obo:IAO_0000115 rdf:datatype="http://www.w3.org/2001/XMLSchema#string">A bounded area of land, or water, usually in its natural or semi-natural (landscaped) state and set aside for some purpose, usually to do with recreation or conservation.</obo:IAO_0000115>
    </owl:Class>
    


    <!-- http://purl.obolibrary.org/obo/ENVO_00000856 -->

    <owl:Class rdf:about="http://purl.obolibrary.org/obo/ENVO_00000856">
        <rdfs:label rdf:datatype="http://www.w3.org/2001/XMLSchema#string">city</rdfs:label>
        <rdfs:subClassOf rdf:resource="http://purl.obolibrary.org/obo/ENVO_01000658"/>
        <obo:IAO_0000115 rdf:datatype="http://www.w3.org/2001/XMLSchema#string">Incorporated populated place.</obo:IAO_0000115>
        <oboInOwl:hasRelatedSynonym rdf:datatype="http://www.w3.org/2001/XMLSchema#string">municipality</oboInOwl:hasRelatedSynonym>
        <oboInOwl:hasRelatedSynonym rdf:datatype="http://www.w3.org/2001/XMLSchema#string">town</oboInOwl:hasRelatedSynonym>
        <oboInOwl:hasRelatedSynonym rdf:datatype="http://www.w3.org/2001/XMLSchema#string">urban area</oboInOwl:hasRelatedSynonym>
        <oboInOwl:hasRelatedSynonym rdf:datatype="http://www.w3.org/2001/XMLSchema#string">village</oboInOwl:hasRelatedSynonym>
    </owl:Class>
    


    <!-- http://purl.obolibrary.org/obo/ENVO_00001999 -->

    <owl:Class rdf:about="http://purl.obolibrary.org/obo/ENVO_00001999">
        <rdfs:label rdf:datatype="http://www.w3.org/2001/XMLSchema#string">marine water body</rdfs:label>
        <rdfs:subClassOf rdf:resource="http://purl.obolibrary.org/obo/ENVO_01000617"/>
        <obo:IAO_0000115 rdf:datatype="http://www.w3.org/2001/XMLSchema#string">A significant accumulation of water which is part of a marine biome.</obo:IAO_0000115>
        <oboInOwl:hasExactSynonym rdf:datatype="http://www.w3.org/2001/XMLSchema#string">body of marine water</oboInOwl:hasExactSynonym>
        <oboInOwl:hasExactSynonym rdf:datatype="http://www.w3.org/2001/XMLSchema#string">marine waterbody</oboInOwl:hasExactSynonym>
    </owl:Class>
    


    <!-- http://purl.obolibrary.org/obo/ENVO_00002001 -->

    <owl:Class rdf:about="http://purl.obolibrary.org/obo/ENVO_00002001">
        <rdfs:label rdf:datatype="http://www.w3.org/2001/XMLSchema#string">waste water</rdfs:label>
        <rdfs:subClassOf rdf:resource="http://purl.obolibrary.org/obo/ENVO_00002186"/>
        <rdfs:subClassOf rdf:resource="http://purl.obolibrary.org/obo/ENVO_00002264"/>
        <obo:IAO_0000115 rdf:datatype="http://www.w3.org/2001/XMLSchema#string">Water that has been adversely affected in quality by anthropogenic influence.</obo:IAO_0000115>
    </owl:Class>
    


    <!-- http://purl.obolibrary.org/obo/ENVO_00002006 -->

    <owl:Class rdf:about="http://purl.obolibrary.org/obo/ENVO_00002006">
        <rdfs:label rdf:datatype="http://www.w3.org/2001/XMLSchema#string">water</rdfs:label>
        <rdfs:subClassOf rdf:resource="http://purl.obolibrary.org/obo/ENVO_00010483"/>
        <obo:IAO_0000115 rdf:datatype="http://www.w3.org/2001/XMLSchema#string">An environmental material primarily composed of dihydrogen oxide in its liquid form.</obo:IAO_0000115>
    </owl:Class>
    


    <!-- http://purl.obolibrary.org/obo/ENVO_00002011 -->

    <owl:Class rdf:about="http://purl.obolibrary.org/obo/ENVO_00002011">
        <rdfs:label rdf:datatype="http://www.w3.org/2001/XMLSchema#string">fresh water</rdfs:label>
        <rdfs:subClassOf rdf:resource="http://purl.obolibrary.org/obo/ENVO_00002006"/>
        <oboInOwl:hasExactSynonym>freshwater</oboInOwl:hasExactSynonym>
    </owl:Class>
    


    <!-- http://purl.obolibrary.org/obo/ENVO_00002018 -->

    <owl:Class rdf:about="http://purl.obolibrary.org/obo/ENVO_00002018">
        <rdfs:label rdf:datatype="http://www.w3.org/2001/XMLSchema#string">sewage</rdfs:label>
        <rdfs:subClassOf rdf:resource="http://purl.obolibrary.org/obo/ENVO_00002001"/>
        <obo:IAO_0000115 rdf:datatype="http://www.w3.org/2001/XMLSchema#string">Wastewater that is contaminated with feces or urine,</obo:IAO_0000115>
    </owl:Class>
    


    <!-- http://purl.obolibrary.org/obo/ENVO_00002186 -->

    <owl:Class rdf:about="http://purl.obolibrary.org/obo/ENVO_00002186">
        <rdfs:label rdf:datatype="http://www.w3.org/2001/XMLSchema#string">contaminated water</rdfs:label>
        <rdfs:subClassOf rdf:resource="http://purl.obolibrary.org/obo/ENVO_00002006"/>
        <oboInOwl:hasExactSynonym rdf:datatype="http://www.w3.org/2001/XMLSchema#string">polluted water</oboInOwl:hasExactSynonym>
    </owl:Class>
    


    <!-- http://purl.obolibrary.org/obo/ENVO_00002193 -->

    <owl:Class rdf:about="http://purl.obolibrary.org/obo/ENVO_00002193">
        <rdfs:label rdf:datatype="http://www.w3.org/2001/XMLSchema#string">pulp-bleaching waste water</rdfs:label>
        <rdfs:subClassOf rdf:resource="http://purl.obolibrary.org/obo/ENVO_00002001"/>
    </owl:Class>
    


    <!-- http://purl.obolibrary.org/obo/ENVO_00002264 -->

    <owl:Class rdf:about="http://purl.obolibrary.org/obo/ENVO_00002264">
        <rdfs:label rdf:datatype="http://www.w3.org/2001/XMLSchema#string">waste material</rdfs:label>
        <rdfs:subClassOf rdf:resource="http://purl.obolibrary.org/obo/ENVO_0010001"/>
        <obo:IAO_0000115>A material which is not the desired output of a process and which is typically the input of a process which removes it from its producer (e.g. a disposal process).</obo:IAO_0000115>
    </owl:Class>
    


    <!-- http://purl.obolibrary.org/obo/ENVO_00002297 -->

    <owl:Class rdf:about="http://purl.obolibrary.org/obo/ENVO_00002297">
        <rdfs:label rdf:datatype="http://www.w3.org/2001/XMLSchema#string">environmental feature</rdfs:label>
        <rdfs:subClassOf rdf:resource="http://purl.obolibrary.org/obo/BFO_0000040"/>
        <obo:IAO_0000115 rdf:datatype="http://www.w3.org/2001/XMLSchema#string">A material entity which determines an environmental system.</obo:IAO_0000115>
    </owl:Class>
    


    <!-- http://purl.obolibrary.org/obo/ENVO_00003064 -->

    <owl:Class rdf:about="http://purl.obolibrary.org/obo/ENVO_00003064">
        <rdfs:label rdf:datatype="http://www.w3.org/2001/XMLSchema#string">drinking water</rdfs:label>
        <rdfs:subClassOf rdf:resource="http://purl.obolibrary.org/obo/ENVO_00002011"/>
        <obo:IAO_0000115>Drinking water is water which may be consumed by humans with no adverse effects on their health.</obo:IAO_0000115>
        <oboInOwl:hasExactSynonym>potable water</oboInOwl:hasExactSynonym>
    </owl:Class>
    


    <!-- http://purl.obolibrary.org/obo/ENVO_00010483 -->

    <owl:Class rdf:about="http://purl.obolibrary.org/obo/ENVO_00010483">
        <rdfs:label rdf:datatype="http://www.w3.org/2001/XMLSchema#string">environmental material</rdfs:label>
        <rdfs:subClassOf rdf:resource="http://purl.obolibrary.org/obo/BFO_0000040"/>
        <obo:IAO_0000115 rdf:datatype="http://www.w3.org/2001/XMLSchema#string">A portion of environmental material is a fiat object which forms the medium or part of the medium of an environmental system.</obo:IAO_0000115>
        <oboInOwl:hasExactSynonym rdf:datatype="http://www.w3.org/2001/XMLSchema#string">portion of environmental material</oboInOwl:hasExactSynonym>
    </owl:Class>
    


    <!-- http://purl.obolibrary.org/obo/ENVO_0010001 -->

    <owl:Class rdf:about="http://purl.obolibrary.org/obo/ENVO_0010001">
        <rdfs:label rdf:datatype="http://www.w3.org/2001/XMLSchema#string">anthropogenic environmental material</rdfs:label>
        <rdfs:subClassOf rdf:resource="http://purl.obolibrary.org/obo/ENVO_00010483"/>
        <obo:IAO_0000115 rdf:datatype="http://www.w3.org/2001/XMLSchema#string">Anthropogenic material in or on which organisms may live.</obo:IAO_0000115>
    </owl:Class>
    


    <!-- http://purl.obolibrary.org/obo/ENVO_01000219 -->

    <owl:Class rdf:about="http://purl.obolibrary.org/obo/ENVO_01000219">
        <rdfs:label rdf:datatype="http://www.w3.org/2001/XMLSchema#string">anthropogenic terrestrial biome</rdfs:label>
        <rdfs:subClassOf rdf:resource="http://purl.obolibrary.org/obo/ENVO_00000446"/>
        <obo:IAO_0000115 rdf:datatype="http://www.w3.org/2001/XMLSchema#string">An anthropogenic terrestrial biome is a terrestrial biome which has community structures determined by human activity.</obo:IAO_0000115>
        <oboInOwl:hasExactSynonym>human biome</oboInOwl:hasExactSynonym>
        <oboInOwl:hasExactSynonym>anthrome</oboInOwl:hasExactSynonym>
    </owl:Class>
    


    <!-- http://purl.obolibrary.org/obo/ENVO_01000245 -->

    <owl:Class rdf:about="http://purl.obolibrary.org/obo/ENVO_01000245">
        <rdfs:label rdf:datatype="http://www.w3.org/2001/XMLSchema#string">cropland biome</rdfs:label>
        <rdfs:subClassOf rdf:resource="http://purl.obolibrary.org/obo/ENVO_01000219"/>
        <obo:IAO_0000115 rdf:datatype="http://www.w3.org/2001/XMLSchema#string">A cropland biome is an anthropogenic terrestrial biome which is primarily used for agricultural activity and which contains no village or larger human settlement.</obo:IAO_0000115>
    </owl:Class>
    


    <!-- http://purl.obolibrary.org/obo/ENVO_01000246 -->

    <owl:Class rdf:about="http://purl.obolibrary.org/obo/ENVO_01000246">
        <rdfs:label rdf:datatype="http://www.w3.org/2001/XMLSchema#string">village biome</rdfs:label>
        <rdfs:subClassOf rdf:resource="http://purl.obolibrary.org/obo/ENVO_01000219"/>
        <obo:IAO_0000115 rdf:datatype="http://www.w3.org/2001/XMLSchema#string">A village biome is an anthropogenic terrestrial biome which contains settlements such as villages, towns, and/or small cities and which is primarily used for agricultural activity.</obo:IAO_0000115>
    </owl:Class>
    


    <!-- http://purl.obolibrary.org/obo/ENVO_01000247 -->

    <owl:Class rdf:about="http://purl.obolibrary.org/obo/ENVO_01000247">
        <rdfs:label rdf:datatype="http://www.w3.org/2001/XMLSchema#string">rangeland biome</rdfs:label>
        <rdfs:subClassOf rdf:resource="http://purl.obolibrary.org/obo/ENVO_01000219"/>
        <obo:IAO_0000115 rdf:datatype="http://www.w3.org/2001/XMLSchema#string">A rangeland biome is an anthropogenic terrestrial biome which is primarily used for the rearing and grazing of livestock.</obo:IAO_0000115>
    </owl:Class>
    


    <!-- http://purl.obolibrary.org/obo/ENVO_01000248 -->

    <owl:Class rdf:about="http://purl.obolibrary.org/obo/ENVO_01000248">
        <rdfs:label rdf:datatype="http://www.w3.org/2001/XMLSchema#string">dense settlement biome</rdfs:label>
        <rdfs:subClassOf rdf:resource="http://purl.obolibrary.org/obo/ENVO_01000219"/>
        <obo:IAO_0000115 rdf:datatype="http://www.w3.org/2001/XMLSchema#string">A dense settlement biome is an anthropogenic terrestrial biome which is primarily used for human habitation, recreation, and industry within built structures with little other land use.</obo:IAO_0000115>
    </owl:Class>
    


    <!-- http://purl.obolibrary.org/obo/ENVO_01000249 -->

    <owl:Class rdf:about="http://purl.obolibrary.org/obo/ENVO_01000249">
        <rdfs:label rdf:datatype="http://www.w3.org/2001/XMLSchema#string">urban biome</rdfs:label>
        <rdfs:subClassOf rdf:resource="http://purl.obolibrary.org/obo/ENVO_01000248"/>
        <obo:IAO_0000115 rdf:datatype="http://www.w3.org/2001/XMLSchema#string">An urban biome is a dense settlement biome which has been urbanised.</obo:IAO_0000115>
    </owl:Class>
    


    <!-- http://purl.obolibrary.org/obo/ENVO_01000254 -->

    <owl:Class rdf:about="http://purl.obolibrary.org/obo/ENVO_01000254">
        <rdfs:label rdf:datatype="http://www.w3.org/2001/XMLSchema#string">environmental system</rdfs:label>
        <rdfs:subClassOf rdf:resource="http://purl.obolibrary.org/obo/RO_0002577"/>
        <obo:IAO_0000115 rdf:datatype="http://www.w3.org/2001/XMLSchema#string">A system which has the disposition to environ one or more material entities.</obo:IAO_0000115>
        <oboInOwl:hasExactSynonym rdf:datatype="http://www.w3.org/2001/XMLSchema#string">environment</oboInOwl:hasExactSynonym>
    </owl:Class>
    


    <!-- http://purl.obolibrary.org/obo/ENVO_01000266 -->

    <owl:Class rdf:about="http://purl.obolibrary.org/obo/ENVO_01000266">
        <rdfs:label rdf:datatype="http://www.w3.org/2001/XMLSchema#string">water vapour</rdfs:label>
        <rdfs:subClassOf rdf:resource="http://purl.obolibrary.org/obo/ENVO_00010483"/>
        <obo:IAO_0000115 rdf:datatype="http://www.w3.org/2001/XMLSchema#string">Water vapour is a vapour which is the gas phase of water.</obo:IAO_0000115>
        <oboInOwl:hasExactSynonym rdf:datatype="http://www.w3.org/2001/XMLSchema#string">aqueous vapor</oboInOwl:hasExactSynonym>
        <oboInOwl:hasExactSynonym rdf:datatype="http://www.w3.org/2001/XMLSchema#string">aqueous vapour</oboInOwl:hasExactSynonym>
        <oboInOwl:hasExactSynonym rdf:datatype="http://www.w3.org/2001/XMLSchema#string">water vapor</oboInOwl:hasExactSynonym>
    </owl:Class>
    


    <!-- http://purl.obolibrary.org/obo/ENVO_01000268 -->

    <owl:Class rdf:about="http://purl.obolibrary.org/obo/ENVO_01000268">
        <rdfs:label rdf:datatype="http://www.w3.org/2001/XMLSchema#string">atmospheric water vapour</rdfs:label>
        <rdfs:subClassOf rdf:resource="http://purl.obolibrary.org/obo/ENVO_01000266"/>
        <obo:IAO_0000115 rdf:datatype="http://www.w3.org/2001/XMLSchema#string">Atmospheric water vapour is water vapour that is part of an atmosphere.</obo:IAO_0000115>
        <oboInOwl:hasExactSynonym rdf:datatype="http://www.w3.org/2001/XMLSchema#string">atmospheric water vapor</oboInOwl:hasExactSynonym>
    </owl:Class>
    


    <!-- http://purl.obolibrary.org/obo/ENVO_01000408 -->

    <owl:Class rdf:about="http://purl.obolibrary.org/obo/ENVO_01000408">
        <rdfs:label>environmental zone</rdfs:label>
        <rdfs:subClassOf rdf:resource="http://purl.obolibrary.org/obo/ENVO_00002297"/>
        <obo:IAO_0000115 rdf:datatype="http://www.w3.org/2001/XMLSchema#string">An environmental zone is an environmental feature whose extent is determined by the presence or influence of one or more material entities or processes. An environmental zone may, itself, assume the role of an environmental feature.</obo:IAO_0000115>
        <oboInOwl:hasRelatedSynonym rdf:datatype="http://www.w3.org/2001/XMLSchema#string">environmental area</oboInOwl:hasRelatedSynonym>
    </owl:Class>
    


    <!-- http://purl.obolibrary.org/obo/ENVO_01000451 -->

    <owl:Class rdf:about="http://purl.obolibrary.org/obo/ENVO_01000451">
        <rdfs:label>atmospheric carbon dioxide</rdfs:label>
        <rdfs:subClassOf rdf:resource="http://purl.obolibrary.org/obo/ENVO_00010483"/>
        <obo:IAO_0000115>Atmospheric carbon dioxide is an environmental material composed of carbon dioxide in its gaseous form present in the atmosphere.</obo:IAO_0000115>
    </owl:Class>
    


    <!-- http://purl.obolibrary.org/obo/ENVO_01000537 -->

    <owl:Class rdf:about="http://purl.obolibrary.org/obo/ENVO_01000537">
        <rdfs:label>atmospheric ozone</rdfs:label>
        <rdfs:subClassOf rdf:resource="http://purl.obolibrary.org/obo/ENVO_00010483"/>
        <oboInOwl:hasRelatedSynonym>atmospheric ozone</oboInOwl:hasRelatedSynonym>
        <obo:IAO_0000115>Atmospheric ozone is an environmental material primarily composed of ozone in its gaseous form and present in the atmosphere.</obo:IAO_0000115>
    </owl:Class>
    


    <!-- http://purl.obolibrary.org/obo/ENVO_01000617 -->

    <owl:Class rdf:about="http://purl.obolibrary.org/obo/ENVO_01000617">
        <rdfs:label xml:lang="en">lentic water body</rdfs:label>
        <rdfs:subClassOf rdf:resource="http://purl.obolibrary.org/obo/ENVO_00000063"/>
        <obo:IAO_0000115>A lentic water body is a water body in which the accumulated water, in its totality, has very little to no directed flow.</obo:IAO_0000115>
    </owl:Class>
    


    <!-- http://purl.obolibrary.org/obo/ENVO_01000618 -->

    <owl:Class rdf:about="http://purl.obolibrary.org/obo/ENVO_01000618">
        <rdfs:label xml:lang="en">lotic water body</rdfs:label>
        <rdfs:subClassOf rdf:resource="http://purl.obolibrary.org/obo/ENVO_00000063"/>
        <obo:IAO_0000115>A lotic water body is a water body in which the accumulated water, in its totality, is flowing.</obo:IAO_0000115>
    </owl:Class>
    


    <!-- http://purl.obolibrary.org/obo/ENVO_01000629 -->

    <owl:Class rdf:about="http://purl.obolibrary.org/obo/ENVO_01000629">
        <rdfs:label xml:lang="en">climate change</rdfs:label>
        <rdfs:subClassOf rdf:resource="http://purl.obolibrary.org/obo/ENVO_02500000"/>
        <obo:IAO_0000115>The long-term fluctuations in temperature, precipitation, wind, and all other aspects of the Earth&apos;s climate. External processes, such as solar-irradiance variations, variations of the Earth&apos;s orbital parameters (eccentricity, precession, and inclination), lithosphere motions, and volcanic activity, are factors in climatic variation. Internal variations of the climate system, e.g., changes in the abundance of greenhouse gases, also may produce fluctuations of sufficient magnitude and variability to explain observed climate change through the feedback processes interrelating the components of the climate system.</obo:IAO_0000115>
    </owl:Class>
    


    <!-- http://purl.obolibrary.org/obo/ENVO_01000634 -->

    <owl:Class rdf:about="http://purl.obolibrary.org/obo/ENVO_01000634">
        <rdfs:label xml:lang="en">volcanic eruption</rdfs:label>
        <rdfs:subClassOf rdf:resource="http://purl.obolibrary.org/obo/ENVO_02500000"/>
        <obo:IAO_0000115>A volcanic process is a process during which lava, tephra (ash, lapilli, volcanic bombs and blocks), and assorted gases are expelled from a volcanic vent or fissure.</obo:IAO_0000115>
    </owl:Class>
    


    <!-- http://purl.obolibrary.org/obo/ENVO_01000653 -->

    <owl:Class rdf:about="http://purl.obolibrary.org/obo/ENVO_01000653">
        <rdfs:label xml:lang="en">slum</rdfs:label>
        <rdfs:subClassOf rdf:resource="http://purl.obolibrary.org/obo/ENVO_01000658"/>
        <obo:IAO_0000115>A slum is a heavily populated urban informal settlement with substandard housing in which households lack any one of the following: access to improved water, access to improved sanitation, sufficient-living area, durability of housing, or security of tenure.</obo:IAO_0000115>
    </owl:Class>
    


    <!-- http://purl.obolibrary.org/obo/ENVO_01000655 -->

    <owl:Class rdf:about="http://purl.obolibrary.org/obo/ENVO_01000655">
        <rdfs:label xml:lang="en">explosive eruption</rdfs:label>
        <rdfs:subClassOf rdf:resource="http://purl.obolibrary.org/obo/ENVO_01000634"/>
        <obo:IAO_0000115>An explosive eruption is a volcanic process in which pressurised magma is violently expelled and froths into volcanic ash. Explosive eruptions can eject a cloud of rocks, dust, gas, and pyroclastic material  which may then collapse, creating a pyroclastic flow of hot volcanic matter.</obo:IAO_0000115>
    </owl:Class>
    


    <!-- http://purl.obolibrary.org/obo/ENVO_01000656 -->

    <owl:Class rdf:about="http://purl.obolibrary.org/obo/ENVO_01000656">
        <rdfs:label xml:lang="en">effusive eruption</rdfs:label>
        <rdfs:subClassOf rdf:resource="http://purl.obolibrary.org/obo/ENVO_01000634"/>
        <obo:IAO_0000115>An effusive eruption is a volcanic eruption during which lava flows onto the ground.</obo:IAO_0000115>
    </owl:Class>
    


    <!-- http://purl.obolibrary.org/obo/ENVO_01000658 -->

    <owl:Class rdf:about="http://purl.obolibrary.org/obo/ENVO_01000658">
        <rdfs:label xml:lang="en">dense settlement</rdfs:label>
        <rdfs:subClassOf rdf:resource="http://purl.obolibrary.org/obo/ENVO_00000062"/>
        <obo:IAO_0000115>A settlement with a high density of buildings and inhabitants.</obo:IAO_0000115>
    </owl:Class>
    


    <!-- http://purl.obolibrary.org/obo/ENVO_01000665 -->

    <owl:Class rdf:about="http://purl.obolibrary.org/obo/ENVO_01000665">
        <rdfs:label xml:lang="en">waste role</rdfs:label>
        <rdfs:subClassOf rdf:resource="http://purl.obolibrary.org/obo/BFO_0000023"/>
        <obo:IAO_0000115>A role that is realized in some process wherein the bearer is discarded or not utilized further.</obo:IAO_0000115>
    </owl:Class>
    


    <!-- http://purl.obolibrary.org/obo/ENVO_01000677 -->

    <owl:Class rdf:about="http://purl.obolibrary.org/obo/ENVO_01000677">
        <rdfs:label xml:lang="en">earthquake</rdfs:label>
        <rdfs:subClassOf rdf:resource="http://purl.obolibrary.org/obo/ENVO_02500000"/>
        <obo:IAO_0000115>An earthquake is a process whereby part of the surface of a planet shakes due to the passage of seismic waves through rocks. Seismic waves are produced when some form of energy stored in a planet&apos;s crust is suddenly released. Elastic strain, gravity, chemical reactions, or even the motion of massive bodies can produce earthquakes.</obo:IAO_0000115>
    </owl:Class>
    


    <!-- http://purl.obolibrary.org/obo/ENVO_01000678 -->

    <owl:Class rdf:about="http://purl.obolibrary.org/obo/ENVO_01000678">
        <rdfs:label xml:lang="en">tectonic earthquake</rdfs:label>
        <rdfs:subClassOf rdf:resource="http://purl.obolibrary.org/obo/ENVO_01000677"/>
        <obo:IAO_0000115>A tectonic earthquake is an earthquake caused by the release of elastic strain. A tectonic earthquake occurs when strains in rock masses have accumulated to a point where the resulting stresses exceed the strength of the rocks, and sudden fracturing results.</obo:IAO_0000115>
    </owl:Class>
    


    <!-- http://purl.obolibrary.org/obo/ENVO_01000679 -->

    <owl:Class rdf:about="http://purl.obolibrary.org/obo/ENVO_01000679">
        <rdfs:label xml:lang="en">megathrust earthquake</rdfs:label>
        <rdfs:subClassOf rdf:resource="http://purl.obolibrary.org/obo/ENVO_01000678"/>
        <obo:IAO_0000115>A megathrust earthquake is a tectonic earthquake which occurs at subduction zones at destructive plate boundaries (convergent boundaries). These interplate earthquakes are the planet&apos;s most powerful, with moment magnitudes that can exceed 9.0.</obo:IAO_0000115>
    </owl:Class>
    


    <!-- http://purl.obolibrary.org/obo/ENVO_01000680 -->

    <owl:Class rdf:about="http://purl.obolibrary.org/obo/ENVO_01000680">
        <rdfs:label xml:lang="en">polluted lake</rdfs:label>
        <rdfs:subClassOf rdf:resource="http://purl.obolibrary.org/obo/ENVO_00000020"/>
        <obo:IAO_0000115>A lake which has concentrations of environmental contaminants high enough to harm the ecosystems associated with it.</obo:IAO_0000115>
    </owl:Class>
    


    <!-- http://purl.obolibrary.org/obo/ENVO_01000687 -->

    <owl:Class rdf:about="http://purl.obolibrary.org/obo/ENVO_01000687">
        <rdfs:label xml:lang="en">coast</rdfs:label>
        <rdfs:subClassOf rdf:resource="http://purl.obolibrary.org/obo/ENVO_00000000"/>
        <obo:IAO_0000115>A coast is the area where land meets the sea, ocean, or lake.</obo:IAO_0000115>
    </owl:Class>
    


    <!-- http://purl.obolibrary.org/obo/ENVO_01000689 -->

    <owl:Class rdf:about="http://purl.obolibrary.org/obo/ENVO_01000689">
        <rdfs:label xml:lang="en">tsunami</rdfs:label>
        <rdfs:subClassOf rdf:resource="http://purl.obolibrary.org/obo/ENVO_02500000"/>
        <oboInOwl:hasExactSynonym>tidal wave</oboInOwl:hasExactSynonym>
        <obo:IAO_0000115>A tsunami is a process during which a series of waves is generated in a water body, typically an ocean or large lake, by the displacement of a large volume of water. Earthquakes, volcanic eruptions and other underwater explosions (including detonations of underwater nuclear devices), landslides, glacier calvings, meteorite impacts and other disturbances above or below water all have the potential to generate a tsunami.</obo:IAO_0000115>
        <oboInOwl:hasExactSynonym>seismic sea wave</oboInOwl:hasExactSynonym>
    </owl:Class>
    


    <!-- http://purl.obolibrary.org/obo/ENVO_01000690 -->

    <owl:Class rdf:about="http://purl.obolibrary.org/obo/ENVO_01000690">
        <rdfs:label xml:lang="en">mass wasting</rdfs:label>
        <rdfs:subClassOf rdf:resource="http://purl.obolibrary.org/obo/ENVO_02500000"/>
        <oboInOwl:hasExactSynonym>slope movement</oboInOwl:hasExactSynonym>
        <oboInOwl:hasBroadSynonym>mass movement</oboInOwl:hasBroadSynonym>
        <obo:IAO_0000115>Mass wasting is the geomorphic process by which solid environmental material such as soil, sand, regolith, and/or rock move downslope typically as a mass, largely under the force of gravity, but frequently affected by water and water content as in submarine environments and mudslides.</obo:IAO_0000115>
    </owl:Class>
    


    <!-- http://purl.obolibrary.org/obo/ENVO_01000691 -->

    <owl:Class rdf:about="http://purl.obolibrary.org/obo/ENVO_01000691">
        <rdfs:label xml:lang="en">avalanche</rdfs:label>
        <rdfs:subClassOf rdf:resource="http://purl.obolibrary.org/obo/ENVO_01000696"/>
        <oboInOwl:hasExactSynonym>snowslip</oboInOwl:hasExactSynonym>
        <obo:IAO_0000115>An avalanche is a rapid flow of snow down a sloping surface.</obo:IAO_0000115>
        <oboInOwl:hasExactSynonym>snowslide</oboInOwl:hasExactSynonym>
    </owl:Class>
    


    <!-- http://purl.obolibrary.org/obo/ENVO_01000692 -->

    <owl:Class rdf:about="http://purl.obolibrary.org/obo/ENVO_01000692">
        <rdfs:label xml:lang="en">landslide process</rdfs:label>
        <rdfs:subClassOf rdf:resource="http://purl.obolibrary.org/obo/ENVO_01000690"/>
        <oboInOwl:hasExactSynonym>landslip</oboInOwl:hasExactSynonym>
        <obo:IAO_0000115>A landslide is a process whereby a large mass of earth and rocks moves down a hill or a mountainside.</obo:IAO_0000115>
    </owl:Class>
    


    <!-- http://purl.obolibrary.org/obo/ENVO_01000693 -->

    <owl:Class rdf:about="http://purl.obolibrary.org/obo/ENVO_01000693">
        <rdfs:label xml:lang="en">rockfall</rdfs:label>
        <rdfs:subClassOf rdf:resource="http://purl.obolibrary.org/obo/ENVO_01000690"/>
    </owl:Class>
    


    <!-- http://purl.obolibrary.org/obo/ENVO_01000694 -->

    <owl:Class rdf:about="http://purl.obolibrary.org/obo/ENVO_01000694">
        <rdfs:label xml:lang="en">geological subsidence</rdfs:label>
        <rdfs:subClassOf rdf:resource="http://purl.obolibrary.org/obo/ENVO_02500000"/>
        <obo:IAO_0000115>A subsidence process is a geomorphologic process in which a surface shifts downward relative to a datum such as sea-level.</obo:IAO_0000115>
        <oboInOwl:hasBroadSynonym>subsidence</oboInOwl:hasBroadSynonym>
    </owl:Class>
    


    <!-- http://purl.obolibrary.org/obo/ENVO_01000695 -->

    <owl:Class rdf:about="http://purl.obolibrary.org/obo/ENVO_01000695">
        <rdfs:label xml:lang="en">mudslide</rdfs:label>
        <rdfs:subClassOf rdf:resource="http://purl.obolibrary.org/obo/ENVO_01000690"/>
    </owl:Class>
    


    <!-- http://purl.obolibrary.org/obo/ENVO_01000696 -->

    <owl:Class rdf:about="http://purl.obolibrary.org/obo/ENVO_01000696">
        <rdfs:label xml:lang="en">mass wasting flow</rdfs:label>
        <rdfs:subClassOf rdf:resource="http://purl.obolibrary.org/obo/ENVO_01000690"/>
        <obo:IAO_0000115>A mass wasting flow is a form of mass wasting during which the moving materials behave similarly to a flowing fluid. Water, air and ice are often involved in enabling fluidlike motion of the material.</obo:IAO_0000115>
        <oboInOwl:hasBroadSynonym>flow</oboInOwl:hasBroadSynonym>
    </owl:Class>
    


    <!-- http://purl.obolibrary.org/obo/ENVO_01000697 -->

    <owl:Class rdf:about="http://purl.obolibrary.org/obo/ENVO_01000697">
        <rdfs:label xml:lang="en">mudflow</rdfs:label>
        <rdfs:subClassOf rdf:resource="http://purl.obolibrary.org/obo/ENVO_01000696"/>
        <obo:IAO_0000115>A mudflow is a form of mass wasting which involves very rapid to extremely rapid surging flow of debris that has become partially or fully liquified by the addition of significant amounts of water to clay-rich source material.</obo:IAO_0000115>
        <oboInOwl:hasExactSynonym>mud flow</oboInOwl:hasExactSynonym>
    </owl:Class>
    


    <!-- http://purl.obolibrary.org/obo/ENVO_01000698 -->

    <owl:Class rdf:about="http://purl.obolibrary.org/obo/ENVO_01000698">
        <rdfs:label xml:lang="en">debris flow</rdfs:label>
        <rdfs:subClassOf rdf:resource="http://purl.obolibrary.org/obo/ENVO_01000696"/>
    </owl:Class>
    


    <!-- http://purl.obolibrary.org/obo/ENVO_01000699 -->

    <owl:Class rdf:about="http://purl.obolibrary.org/obo/ENVO_01000699">
        <rdfs:label xml:lang="en">lahar</rdfs:label>
        <rdfs:subClassOf rdf:resource="http://purl.obolibrary.org/obo/ENVO_01000697"/>
        <obo:IAO_0000115>A lahar is a type of mudflow or debris flow composed of a slurry of pyroclastic material, rocky debris, and water. The material flows down from a volcano, typically along a river valley.</obo:IAO_0000115>
    </owl:Class>
    


    <!-- http://purl.obolibrary.org/obo/ENVO_01000700 -->

    <owl:Class rdf:about="http://purl.obolibrary.org/obo/ENVO_01000700">
        <rdfs:label xml:lang="en">sturzstrom</rdfs:label>
        <rdfs:subClassOf rdf:resource="http://purl.obolibrary.org/obo/ENVO_01000692"/>
        <obo:IAO_0000115>A sturzstrom is a landslide consisting which has a great amount of kinetic energy resulting in greater horizontal movement when compared to its initial vertical drop â€” as much as 20 or 30 times the vertical distance. By contrast a normal landslide will typically travel a horizontal distance that is less than twice the distance that the material has fallen.</obo:IAO_0000115>
    </owl:Class>
    


    <!-- http://purl.obolibrary.org/obo/ENVO_01000702 -->

    <owl:Class rdf:about="http://purl.obolibrary.org/obo/ENVO_01000702">
        <rdfs:label xml:lang="en">ash fall process</rdfs:label>
        <rdfs:subClassOf rdf:resource="http://purl.obolibrary.org/obo/ENVO_02500000"/>
        <obo:IAO_0000115>An ash fall process is a process in which volcanic ash formed during an explosive volcanic eruption, phreatomagmatic eruption, or during material transport in pyroclastic density currents is pulled towards the planetary surface by gravity.</obo:IAO_0000115>
    </owl:Class>
    


    <!-- http://purl.obolibrary.org/obo/ENVO_01000707 -->

    <owl:Class rdf:about="http://purl.obolibrary.org/obo/ENVO_01000707">
        <rdfs:label xml:lang="en">coastal flooding</rdfs:label>
        <rdfs:subClassOf rdf:resource="http://purl.obolibrary.org/obo/ENVO_02500002"/>
        <obo:IAO_0000115>Coastal flooding is a process in which normally dry, low-lying land near a coast is flooded by sea water.</obo:IAO_0000115>
    </owl:Class>
    


    <!-- http://purl.obolibrary.org/obo/ENVO_01000708 -->

    <owl:Class rdf:about="http://purl.obolibrary.org/obo/ENVO_01000708">
        <rdfs:label xml:lang="en">riverine flooding</rdfs:label>
        <rdfs:subClassOf rdf:resource="http://purl.obolibrary.org/obo/ENVO_02500002"/>
        <obo:IAO_0000115>Riverine flooding is a process in which the flow rate of river water exceeds the capacity of its channel, thus flooding neighbouring land. Bends and meanders in a river channel are particularly disposed to such flooding.</obo:IAO_0000115>
    </owl:Class>
    


    <!-- http://purl.obolibrary.org/obo/ENVO_01000709 -->

    <owl:Class rdf:about="http://purl.obolibrary.org/obo/ENVO_01000709">
        <rdfs:label xml:lang="en">flash flooding</rdfs:label>
        <rdfs:subClassOf rdf:resource="http://purl.obolibrary.org/obo/ENVO_02500002"/>
        <obo:IAO_0000115>Flash flooding is a process in which low-lying land is inundated with water for a short period of time and are usually the result of precipitation or a breach in the container of a water body.</obo:IAO_0000115>
    </owl:Class>
    


    <!-- http://purl.obolibrary.org/obo/ENVO_01000710 -->

    <owl:Class rdf:about="http://purl.obolibrary.org/obo/ENVO_01000710">
        <rdfs:label xml:lang="en">flood</rdfs:label>
        <rdfs:subClassOf rdf:resource="http://purl.obolibrary.org/obo/ENVO_00000063"/>
        <obo:IAO_0000115>An unusual accumulation of water above the ground caused by high tide, heavy rain, melting snow or rapid runoff from paved areas.</obo:IAO_0000115>
    </owl:Class>
    


    <!-- http://purl.obolibrary.org/obo/ENVO_01000711 -->

    <owl:Class rdf:about="http://purl.obolibrary.org/obo/ENVO_01000711">
        <rdfs:label xml:lang="en">coastal flood</rdfs:label>
        <rdfs:subClassOf rdf:resource="http://purl.obolibrary.org/obo/ENVO_01000710"/>
        <obo:IAO_0000115>A coastal flood is a flood which is formed as a result of large amounts of water from marine water bodies or large lakes being transported to usually dry land by displacement processes such as high winds or seismic activity.</obo:IAO_0000115>
    </owl:Class>
    


    <!-- http://purl.obolibrary.org/obo/ENVO_01000712 -->

    <owl:Class rdf:about="http://purl.obolibrary.org/obo/ENVO_01000712">
        <rdfs:label xml:lang="en">riverine flood</rdfs:label>
        <rdfs:subClassOf rdf:resource="http://purl.obolibrary.org/obo/ENVO_01000710"/>
        <obo:IAO_0000115>A riverine flood is a flood which is formed as a result of a river&apos;s flow rate exceeding the capacity of its channel.</obo:IAO_0000115>
    </owl:Class>
    


    <!-- http://purl.obolibrary.org/obo/ENVO_01000713 -->

    <owl:Class rdf:about="http://purl.obolibrary.org/obo/ENVO_01000713">
        <rdfs:label xml:lang="en">flash flood</rdfs:label>
        <rdfs:subClassOf rdf:resource="http://purl.obolibrary.org/obo/ENVO_01000710"/>
        <obo:IAO_0000115>A flash flood is a flood formed by the rapid flooding of geomorphic low-lying areas. It may be caused by heavy rain associated with a severe thunderstorm, hurricane, tropical storm, or meltwater from ice or snow flowing over ice sheets or snowfields. Flash floods may also occur after the collapse of a natural ice or debris dam, or a human structure such as a man-made dam. Flash floods are distinguished from a regular flood by a timescale of less than six hours.</obo:IAO_0000115>
    </owl:Class>
    


    <!-- http://purl.obolibrary.org/obo/ENVO_01000714 -->

    <owl:Class rdf:about="http://purl.obolibrary.org/obo/ENVO_01000714">
        <rdfs:label xml:lang="en">storm surge</rdfs:label>
        <rdfs:subClassOf rdf:resource="http://purl.obolibrary.org/obo/ENVO_01000711"/>
        <obo:IAO_0000115>A storm surge is a coastal flood which is caused by low-pressure weather systems such as tropical cyclones and strong extratropical cyclones, the severity of which is affected by the shallowness and orientation of the water body relative to storm path, and the timing of tides.</obo:IAO_0000115>
    </owl:Class>
    


    <!-- http://purl.obolibrary.org/obo/ENVO_01000715 -->

    <owl:Class rdf:about="http://purl.obolibrary.org/obo/ENVO_01000715">
        <rdfs:label xml:lang="en">metotsunami</rdfs:label>
        <rdfs:subClassOf rdf:resource="http://purl.obolibrary.org/obo/ENVO_01000689"/>
        <obo:IAO_0000115>A meteotsunami is a tsunami caused by atmospheric processes and differences in air pressure.</obo:IAO_0000115>
    </owl:Class>
    


    <!-- http://purl.obolibrary.org/obo/ENVO_01000716 -->

    <owl:Class rdf:about="http://purl.obolibrary.org/obo/ENVO_01000716">
        <rdfs:label xml:lang="en">storm surge process</rdfs:label>
        <rdfs:subClassOf rdf:resource="http://purl.obolibrary.org/obo/ENVO_01000707"/>
        <obo:IAO_0000115>A storm surge process is a coastal flooding process which is caused by low pressure weather systems such as tropical cyclones and strong extratropical cyclones, the severity of which is affected by the shallowness and orientation of the water body relative to storm path, and the timing of tides.</obo:IAO_0000115>
    </owl:Class>
    


    <!-- http://purl.obolibrary.org/obo/ENVO_01000717 -->

    <owl:Class rdf:about="http://purl.obolibrary.org/obo/ENVO_01000717">
        <rdfs:label xml:lang="en">areal flooding</rdfs:label>
        <rdfs:subClassOf rdf:resource="http://purl.obolibrary.org/obo/ENVO_02500002"/>
        <obo:IAO_0000115>Areal flooding is a flooding process in which flat or low-lying areas become inundated with water due to water input exceeding infiltration, evaporation, or run off.</obo:IAO_0000115>
    </owl:Class>
    


    <!-- http://purl.obolibrary.org/obo/ENVO_01000718 -->

    <owl:Class rdf:about="http://purl.obolibrary.org/obo/ENVO_01000718">
        <rdfs:label xml:lang="en">urban flooding</rdfs:label>
        <rdfs:subClassOf rdf:resource="http://purl.obolibrary.org/obo/ENVO_02500002"/>
        <obo:IAO_0000115>Urban flooding is a flooding process in which land or property in a built environment, particularly in more densely populated areas, is inundated due to the rate of water input exceeding that of water drainage provided by the environment&apos;s drainage systems.</obo:IAO_0000115>
    </owl:Class>
    


    <!-- http://purl.obolibrary.org/obo/ENVO_01000730 -->

    <owl:Class rdf:about="http://purl.obolibrary.org/obo/ENVO_01000730">
        <rdfs:label xml:lang="en">lava flow process</rdfs:label>
        <rdfs:subClassOf rdf:resource="http://purl.obolibrary.org/obo/ENVO_02500000"/>
        <obo:IAO_0000115>A process in which a volume of lava emitted during an effusive eruption moves along a solid surface.</obo:IAO_0000115>
    </owl:Class>
    


    <!-- http://purl.obolibrary.org/obo/ENVO_01000741 -->

    <owl:Class rdf:about="http://purl.obolibrary.org/obo/ENVO_01000741">
        <rdfs:label xml:lang="en">recycling process</rdfs:label>
        <rdfs:subClassOf rdf:resource="http://purl.obolibrary.org/obo/ENVO_02500000"/>
        <obo:IAO_0000115>A process in which has inputs which bear waste roles and outputs which bear resource roles.</obo:IAO_0000115>
    </owl:Class>
    


    <!-- http://purl.obolibrary.org/obo/ENVO_01000742 -->

    <owl:Class rdf:about="http://purl.obolibrary.org/obo/ENVO_01000742">
        <rdfs:label xml:lang="en">carbon-bearing gas emission process</rdfs:label>
        <rdfs:subClassOf rdf:resource="http://purl.obolibrary.org/obo/ENVO_02500000"/>
        <obo:IAO_0000115>A carbon emission process is any environmental process which outputs a carbon-bearing gas.</obo:IAO_0000115>
        <oboInOwl:hasBroadSynonym>carbon emission process</oboInOwl:hasBroadSynonym>
    </owl:Class>
    


    <!-- http://purl.obolibrary.org/obo/ENVO_01000743 -->

    <owl:Class rdf:about="http://purl.obolibrary.org/obo/ENVO_01000743">
        <rdfs:label xml:lang="en">land consumption process</rdfs:label>
        <rdfs:subClassOf rdf:resource="http://purl.obolibrary.org/obo/ENVO_02500005"/>
        <obo:IAO_0000115>A process in which natural ecosystems present over an expanse of land are removed and replaced with anthropogenic ecosystems.</obo:IAO_0000115>
    </owl:Class>
    


    <!-- http://purl.obolibrary.org/obo/ENVO_01000744 -->

    <owl:Class rdf:about="http://purl.obolibrary.org/obo/ENVO_01000744">
        <rdfs:label xml:lang="en">human dwelling</rdfs:label>
        <rdfs:subClassOf rdf:resource="http://purl.obolibrary.org/obo/ENVO_00000070"/>
        <obo:IAO_0000115>A self-contained constructed feature used by one or more households as a home, such as a house, apartment, mobile home, houseboat or other &apos;substantial&apos; structure. A dwelling typically includes nearby outbuildings, sheds etc. within the curtilage of the property, excluding any &apos;open fields beyond&apos;. It has significance in relation to search and seizure, conveyancing of real property, burglary, trespass, and land use planning.</obo:IAO_0000115>
    </owl:Class>
    


    <!-- http://purl.obolibrary.org/obo/ENVO_01000762 -->

    <owl:Class rdf:about="http://purl.obolibrary.org/obo/ENVO_01000762">
        <rdfs:label xml:lang="en">sparsely populated settlement</rdfs:label>
        <rdfs:subClassOf rdf:resource="http://purl.obolibrary.org/obo/ENVO_00000062"/>
        <obo:IAO_0000115>A settlement with a low density of buildings and inhabitants.</obo:IAO_0000115>
    </owl:Class>
    


    <!-- http://purl.obolibrary.org/obo/ENVO_01000763 -->

    <owl:Class rdf:about="http://purl.obolibrary.org/obo/ENVO_01000763">
        <rdfs:label xml:lang="en">rural settlement</rdfs:label>
        <rdfs:subClassOf rdf:resource="http://purl.obolibrary.org/obo/ENVO_01000762"/>
        <obo:IAO_0000115>A settlement which has lower population density than a town, city, or other urban environment and is primarily used for agricultural or pastoral activity.</obo:IAO_0000115>
    </owl:Class>
    


    <!-- http://purl.obolibrary.org/obo/ENVO_01000764 -->

    <owl:Class rdf:about="http://purl.obolibrary.org/obo/ENVO_01000764">
        <rdfs:label xml:lang="en">formal settlement</rdfs:label>
        <rdfs:subClassOf rdf:resource="http://purl.obolibrary.org/obo/ENVO_00000062"/>
        <obo:IAO_0000115>A settlement which has been established and is managed through officially sanctioned processes and is recognised as legal by a competent authority.</obo:IAO_0000115>
    </owl:Class>
    


    <!-- http://purl.obolibrary.org/obo/ENVO_01000765 -->

    <owl:Class rdf:about="http://purl.obolibrary.org/obo/ENVO_01000765">
        <rdfs:label xml:lang="en">informal settlement</rdfs:label>
        <rdfs:subClassOf rdf:resource="http://purl.obolibrary.org/obo/ENVO_00000062"/>
        <obo:IAO_0000115>A settlement which is not associated with or directed by official planning processes and which typically lacks municipal services and infrastructure such as sanitation, water services, and waste management services.</obo:IAO_0000115>
    </owl:Class>
    


    <!-- http://purl.obolibrary.org/obo/ENVO_01000767 -->

    <owl:Class rdf:about="http://purl.obolibrary.org/obo/ENVO_01000767">
        <rdfs:label xml:lang="en">illegal settlement</rdfs:label>
        <rdfs:subClassOf rdf:resource="http://purl.obolibrary.org/obo/ENVO_00000062"/>
        <obo:IAO_0000115>A settlement on land that the inhabitants have no legal claim to or occupy illegally.</obo:IAO_0000115>
    </owl:Class>
    


    <!-- http://purl.obolibrary.org/obo/ENVO_01000769 -->

    <owl:Class rdf:about="http://purl.obolibrary.org/obo/ENVO_01000769">
        <rdfs:label xml:lang="en">carbon dioxide emission process</rdfs:label>
        <rdfs:subClassOf rdf:resource="http://purl.obolibrary.org/obo/ENVO_01000742"/>
        <obo:IAO_0000115>A carbon emission process is any environmental process which releases carbon dioxide gas into the atmosphere.</obo:IAO_0000115>
    </owl:Class>
    


    <!-- http://purl.obolibrary.org/obo/ENVO_01000770 -->

    <owl:Class rdf:about="http://purl.obolibrary.org/obo/ENVO_01000770">
        <rdfs:label xml:lang="en">cabon dioxide emission</rdfs:label>
        <rdfs:subClassOf rdf:resource="http://purl.obolibrary.org/obo/ENVO_00010483"/>
        <obo:IAO_0000115>A volume of carbon dioxide gas emitted by a carbon dioxide emission process.</obo:IAO_0000115>
    </owl:Class>
    


    <!-- http://purl.obolibrary.org/obo/ENVO_01000772 -->

    <owl:Class rdf:about="http://purl.obolibrary.org/obo/ENVO_01000772">
        <rdfs:label xml:lang="en">rural area</rdfs:label>
        <rdfs:subClassOf rdf:resource="http://purl.obolibrary.org/obo/ENVO_01000408"/>
        <obo:IAO_0000115>An area which is outside of a town, city, or urban area. Rural areas are primarily used for agriculture or pastoralism and may contain rural settlements.</obo:IAO_0000115>
    </owl:Class>
    


    <!-- http://purl.obolibrary.org/obo/ENVO_01000773 -->

    <owl:Class rdf:about="http://purl.obolibrary.org/obo/ENVO_01000773">
        <rdfs:label xml:lang="en">village</rdfs:label>
        <rdfs:subClassOf rdf:resource="http://purl.obolibrary.org/obo/ENVO_00000062"/>
        <obo:IAO_0000115>A village is a clustered human settlement or community, larger than a hamlet but smaller than a town, with a population ranging from a few hundred to a few thousand. Though often located in rural areas, the term urban village is also applied to certain urban neighbourhoods. Villages are normally permanent, with fixed dwellings; however, transient villages can occur. Further, the dwellings of a village are fairly close to one another, not scattered broadly over the landscape, as a dispersed settlement.</obo:IAO_0000115>
    </owl:Class>
    


    <!-- http://purl.obolibrary.org/obo/ENVO_01000778 -->

    <owl:Class rdf:about="http://purl.obolibrary.org/obo/ENVO_01000778">
        <rdfs:label xml:lang="en">important site</rdfs:label>
        <rdfs:subClassOf rdf:resource="http://purl.obolibrary.org/obo/ENVO_01000408"/>
        <rdfs:subClassOf rdf:resource="http://purl.obolibrary.org/obo/PCO_0000002"/>
        <oboInOwl:hasNarrowSynonym>Ramsar Sites</oboInOwl:hasNarrowSynonym>
        <oboInOwl:hasNarrowSynonym>Important Mammal Area</oboInOwl:hasNarrowSynonym>
        <oboInOwl:hasNarrowSynonym>Prime Butterfly Area</oboInOwl:hasNarrowSynonym>
        <oboInOwl:hasNarrowSynonym>Ecologically and Biologically Significant Area</oboInOwl:hasNarrowSynonym>
        <oboInOwl:hasNarrowSynonym>Alliance for Zero Extinction Sites</oboInOwl:hasNarrowSynonym>
        <oboInOwl:hasNarrowSynonym>IUCN Important Site for Freshwater Biodiversity</oboInOwl:hasNarrowSynonym>
        <oboInOwl:hasNarrowSynonym>Important Bird Area</oboInOwl:hasNarrowSynonym>
        <oboInOwl:hasExactSynonym>key biodiversity area</oboInOwl:hasExactSynonym>
        <oboInOwl:hasNarrowSynonym>Important Plant Area</oboInOwl:hasNarrowSynonym>
        <obo:IAO_0000115>An environmental zone which contains, as determined by an officially mandated selection process, one or more ecosystems which include, as parts, ecological communities of global significance for conservation due to their vulnerability and irreplaceability.</obo:IAO_0000115>
        <oboInOwl:hasNarrowSynonym>Important Site for Freshwater Biodiversity</oboInOwl:hasNarrowSynonym>
    </owl:Class>
    


    <!-- http://purl.obolibrary.org/obo/ENVO_02500000 -->

    <owl:Class rdf:about="http://purl.obolibrary.org/obo/ENVO_02500000">
        <rdfs:label xml:lang="en">environmental system process</rdfs:label>
        <rdfs:subClassOf rdf:resource="http://purl.obolibrary.org/obo/BFO_0000015"/>
    </owl:Class>
    


    <!-- http://purl.obolibrary.org/obo/ENVO_02500001 -->

    <owl:Class rdf:about="http://purl.obolibrary.org/obo/ENVO_02500001">
        <rdfs:label xml:lang="en">desertification</rdfs:label>
        <rdfs:subClassOf rdf:resource="http://purl.obolibrary.org/obo/ENVO_02500000"/>
        <obo:IAO_0000115>a type of land degradation in which a relatively dry land region becomes increasingly arid, typically losing its bodies of water as well as vegetation and wildlife.</obo:IAO_0000115>
    </owl:Class>
    


    <!-- http://purl.obolibrary.org/obo/ENVO_02500002 -->

    <owl:Class rdf:about="http://purl.obolibrary.org/obo/ENVO_02500002">
        <rdfs:label xml:lang="en">flooding</rdfs:label>
        <rdfs:subClassOf rdf:resource="http://purl.obolibrary.org/obo/ENVO_02500000"/>
        <obo:IAO_0000115>A general and temporary condition of partial or complete inundation of normally dry land areas from the overflow of inland and/or tidal waters, and/or the unusual and rapid accumulation or runoff of surface waters from any source. A great flow along a watercourse or a flow causing inundation of lands not normally covered by water.</obo:IAO_0000115>
    </owl:Class>
    


    <!-- http://purl.obolibrary.org/obo/ENVO_02500005 -->

    <owl:Class rdf:about="http://purl.obolibrary.org/obo/ENVO_02500005">
        <rdfs:label>land degradation</rdfs:label>
        <rdfs:subClassOf rdf:resource="http://purl.obolibrary.org/obo/ENVO_02500000"/>
        <obo:IAO_0000115>A process which diminishes the functioning of an ecosystem located on land.</obo:IAO_0000115>
    </owl:Class>
    


    <!-- http://purl.obolibrary.org/obo/ENVO_02500011 -->

    <owl:Class rdf:about="http://purl.obolibrary.org/obo/ENVO_02500011">
        <rdfs:label>afforestation</rdfs:label>
        <rdfs:subClassOf rdf:resource="http://purl.obolibrary.org/obo/ENVO_02500000"/>
        <obo:IAO_0000115>Establishment of a new forest by seeding or planting of nonforested land.</obo:IAO_0000115>
    </owl:Class>
    


    <!-- http://purl.obolibrary.org/obo/ENVO_02500012 -->

    <owl:Class rdf:about="http://purl.obolibrary.org/obo/ENVO_02500012">
        <rdfs:label>deforestation</rdfs:label>
        <rdfs:subClassOf rdf:resource="http://purl.obolibrary.org/obo/ENVO_02500000"/>
        <oboInOwl:hasBroadSynonym>clearance</oboInOwl:hasBroadSynonym>
        <obo:IAO_0000115>The removal of forest and undergrowth to, for example, increase the surface of arable land or to use the timber for construction or industrial purposes.</obo:IAO_0000115>
        <oboInOwl:hasBroadSynonym>clearing</oboInOwl:hasBroadSynonym>
    </owl:Class>
    


    <!-- http://purl.obolibrary.org/obo/ENVO_02500013 -->

    <owl:Class rdf:about="http://purl.obolibrary.org/obo/ENVO_02500013">
        <rdfs:label>reforestation</rdfs:label>
        <rdfs:subClassOf rdf:resource="http://purl.obolibrary.org/obo/ENVO_02500032"/>
        <obo:IAO_0000115>The planting of trees in areas in where forests have previously been cleared.</obo:IAO_0000115>
    </owl:Class>
    


    <!-- http://purl.obolibrary.org/obo/ENVO_02500017 -->

    <owl:Class rdf:about="http://purl.obolibrary.org/obo/ENVO_02500017">
        <rdfs:label>anthropogenic reforestation</rdfs:label>
        <rdfs:subClassOf rdf:resource="http://purl.obolibrary.org/obo/ENVO_02500013"/>
        <rdfs:subClassOf rdf:resource="http://purl.obolibrary.org/obo/ENVO_02500027"/>
    </owl:Class>
    


    <!-- http://purl.obolibrary.org/obo/ENVO_02500027 -->

    <owl:Class rdf:about="http://purl.obolibrary.org/obo/ENVO_02500027">
        <rdfs:label>anthropogenic environmental process</rdfs:label>
        <rdfs:subClassOf rdf:resource="http://purl.obolibrary.org/obo/ENVO_02500000"/>
    </owl:Class>
    


    <!-- http://purl.obolibrary.org/obo/ENVO_02500032 -->

    <owl:Class rdf:about="http://purl.obolibrary.org/obo/ENVO_02500032">
        <rdfs:label>revegetation</rdfs:label>
        <rdfs:subClassOf rdf:resource="http://purl.obolibrary.org/obo/ENVO_02500000"/>
    </owl:Class>
    


    <!-- http://purl.obolibrary.org/obo/PCO_0000000 -->

    <owl:Class rdf:about="http://purl.obolibrary.org/obo/PCO_0000000">
        <rdfs:label rdf:datatype="http://www.w3.org/2001/XMLSchema#string">collection of organisms</rdfs:label>
        <rdfs:subClassOf rdf:resource="http://purl.obolibrary.org/obo/BFO_0000040"/>
        <obo:IAO_0000115 rdf:datatype="http://www.w3.org/2001/XMLSchema#string">A material entity that consists of two or more organisms, viruses, or viroids.</obo:IAO_0000115>
    </owl:Class>
    


    <!-- http://purl.obolibrary.org/obo/PCO_0000002 -->

    <owl:Class rdf:about="http://purl.obolibrary.org/obo/PCO_0000002">
        <rdfs:label rdf:datatype="http://www.w3.org/2001/XMLSchema#string">ecological community</rdfs:label>
        <rdfs:subClassOf rdf:resource="http://purl.obolibrary.org/obo/PCO_0000000"/>
        <obo:IAO_0000115 rdf:datatype="http://www.w3.org/2001/XMLSchema#string">A collection of organisms of at least two different species, living in a particular area.</obo:IAO_0000115>
    </owl:Class>
    


    <!-- http://purl.obolibrary.org/obo/RO_0002577 -->

    <owl:Class rdf:about="http://purl.obolibrary.org/obo/RO_0002577">
        <rdfs:label>system</rdfs:label>
        <rdfs:subClassOf rdf:resource="http://purl.obolibrary.org/obo/BFO_0000040"/>
        <obo:IAO_0000115>A material entity consisting of multiple components that are causally integrated.</obo:IAO_0000115>
    </owl:Class>
</rdf:RDF>



<!-- Generated by the OWL API (version 0.0.1+6049ab4) http://owlapi.sourceforge.net -->

