format-version: 1.2
ontology: http://purl.unep.org/sdg/imports/envo_import.owl

[Term]
id: BFO:0000002
name: continuant
def: "An entity that exists in full at any time in which it exists at all, persists through time while maintaining its identity and has no temporal parts." []
disjoint_from: BFO:0000003 ! occurrent

[Term]
id: BFO:0000003
name: occurrent
def: "An entity that has temporal parts and that happens, unfolds or develops through time." []

[Term]
id: BFO:0000004
name: independent continuant
def: "A continuant that is a bearer of quality and realizable entity entities, in which other entities inhere and which itself cannot inhere in anything." []
is_a: BFO:0000002 ! continuant
disjoint_from: BFO:0000020 ! specifically dependent continuant

[Term]
id: BFO:0000015
name: process
def: "An occurrent that has temporal proper parts and for some time t, p s-depends_on some material entity at t." []
is_a: BFO:0000003 ! occurrent

[Term]
id: BFO:0000017
name: realizable entity
def: "A specifically dependent continuant  that inheres in continuant  entities and are not exhibited in full at every time in which it inheres in an entity or group of entities. The exhibition or actualization of a realizable entity is a particular manifestation, functioning or process that occurs under certain circumstances." []
is_a: BFO:0000020 ! specifically dependent continuant

[Term]
id: BFO:0000020
name: specifically dependent continuant
def: "A continuant that inheres in or is borne by other entities. Every instance of A requires some specific instance of B which must always be the same." []
is_a: BFO:0000002 ! continuant

[Term]
id: BFO:0000023
name: role
def: "A realizable entity  the manifestation of which brings about some result or end that is not essential to a continuant  in virtue of the kind of thing that it is but that can be served or participated in by that kind of continuant  in some kinds of natural, social or institutional contexts." []
is_a: BFO:0000017 ! realizable entity

[Term]
id: BFO:0000040
name: material entity
def: "An independent continuant that is spatially extended whose identity is independent of that of other entities and can be maintained through time." []
is_a: BFO:0000004 ! independent continuant

[Term]
id: ENVO:00000000
name: geographic feature
synonym: "macroscopic spatial feature" EXACT []
is_a: ENVO:00002297 ! environmental feature

[Term]
id: ENVO:00000002
name: anthropogenic geographic feature
def: "An anthropogenic geographic feature is a geographic feature\nresulting from the influence of human beings on nature." []
synonym: "man-made feature" RELATED []
synonym: "manmade feature" RELATED []
is_a: ENVO:00000000 ! geographic feature

[Term]
id: ENVO:00000004
name: administrative region
synonym: "administrative area" EXACT []
synonym: "administrative division" RELATED []
synonym: "administrative entity" RELATED []
synonym: "boundary region" RELATED []
synonym: "civil area" RELATED []
synonym: "district" RELATED []
synonym: "free trade zone" RELATED []
synonym: "governed place" RELATED []
synonym: "leased area (government)" RELATED []
synonym: "leased zone (government)" RELATED []
synonym: "neutral zone (political)" RELATED []
synonym: "prefecture" RELATED []
synonym: "protectorate" RELATED []
synonym: "sheikdom" RELATED []
synonym: "sultanate" RELATED []
synonym: "trade zone" RELATED []
is_a: ENVO:00000002 ! anthropogenic geographic feature

[Term]
id: ENVO:00000005
name: first-order administrative region
def: "A primary administrative division of a country, such as a state in the United States." []
synonym: "countries, 1st order division" RELATED []
synonym: "first level subdivision" RELATED []
synonym: "first-order administrative division" RELATED []
is_a: ENVO:00000004 ! administrative region

[Term]
id: ENVO:00000006
name: second-order administrative region
def: "A subdivision of a first-order administrative division." []
synonym: "countries, 2nd order division" RELATED []
synonym: "second level subdivision" RELATED []
synonym: "second-order administrative division" RELATED []
is_a: ENVO:00000004 ! administrative region

[Term]
id: ENVO:00000007
name: third-order administrative region
def: "A subdivision of a second-order administrative division." []
synonym: "barrio" RELATED []
synonym: "countries, 3rd order division" RELATED []
synonym: "third level subdivision" RELATED []
synonym: "third-order administrative division" RELATED []
is_a: ENVO:00000004 ! administrative region

[Term]
id: ENVO:00000008
name: fourth-order administrative region
def: "A subdivision of a third-order administrative division." []
synonym: "countries, 4th order division" RELATED []
synonym: "fourth level subdivision" RELATED []
synonym: "fourth-order administrative division" RELATED []
is_a: ENVO:00000004 ! administrative region

[Term]
id: ENVO:00000009
name: national geopolitical entity
def: "A political association with effective dominion over a geographic area." []
synonym: "country" RELATED []
synonym: "independent nation" NARROW []
synonym: "independent political entity" NARROW []
synonym: "independent sovereign nation" NARROW []
synonym: "nation" EXACT []
synonym: "political entity" RELATED []
synonym: "state" RELATED []
is_a: ENVO:00000123 ! political entity

[Term]
id: ENVO:00000015
name: ocean
def: "Continuous saline-water bodies that surround the continents and fill the Earth's great depressions." []
synonym: "Ocean" EXACT []
synonym: "ocean" EXACT []
synonym: "ocean region" RELATED []
synonym: "sea" RELATED []
is_a: ENVO:00001999 ! marine water body

[Term]
id: ENVO:00000016
name: sea
def: "A large expanse of saline water usually connected with an ocean." []
synonym: "channel" NARROW []
synonym: "closed sea" NARROW []
synonym: "marginal sea" NARROW []
synonym: "open sea" NARROW []
synonym: "open sound" NARROW []
synonym: "open water" NARROW []
synonym: "Sea" EXACT []
synonym: "sea" EXACT []
is_a: ENVO:00001999 ! marine water body

[Term]
id: ENVO:00000020
name: lake
def: "A body of water or other liquid of considerable size contained on a body of land." []
synonym: "broad" RELATED []
synonym: "catch basin" NARROW []
synonym: "llyn" RELATED []
synonym: "loch" RELATED []
synonym: "lochan" RELATED []
synonym: "lough" RELATED []
synonym: "mere" RELATED []
synonym: "mortlake" RELATED []
synonym: "open water" NARROW []
synonym: "pasteuer lake" RELATED []
synonym: "tarn" NARROW []
is_a: ENVO:01000617 ! lentic water body

[Term]
id: ENVO:00000022
name: river
def: "Natural freshwater surface streams of considerable volume and a permanent or seasonal flow, moving in a definite channel toward a sea, lake, or another river; any large streams, or ones larger than brooks or creeks, such as the trunk stream and larger branches of a drainage system." []
synonym: "braided river" NARROW []
synonym: "rio" EXACT []
is_a: ENVO:00000023 ! stream

[Term]
id: ENVO:00000023
name: stream
def: "Linear body of water flowing on the Earth's surface." []
synonym: "beck" RELATED []
synonym: "braided stream" NARROW []
synonym: "brook" RELATED []
synonym: "burn (hydrographic)" RELATED []
synonym: "Creek" RELATED []
synonym: "creek" RELATED []
synonym: "fork (hydrographic" NARROW []
synonym: "glacial stream" NARROW []
synonym: "lode" NARROW []
synonym: "millstream" NARROW []
synonym: "rivulet" RELATED []
synonym: "Stream" EXACT []
synonym: "stream" EXACT []
synonym: "stream bend" NARROW []
synonym: "streams" EXACT []
synonym: "watercourse" BROAD []
is_a: ENVO:00000029 ! watercourse

[Term]
id: ENVO:00000029
name: watercourse
def: "A flowing body of water." []
synonym: "awawa" RELATED []
synonym: "barranca" RELATED []
synonym: "beck" RELATED []
synonym: "branch" RELATED []
synonym: "brook" RELATED []
synonym: "course" RELATED []
synonym: "culvert" NARROW []
synonym: "draw" RELATED []
synonym: "dredged channel" NARROW []
synonym: "fork" NARROW []
synonym: "gulch" NARROW []
synonym: "gully" NARROW []
synonym: "gut" NARROW []
synonym: "gutter" NARROW []
synonym: "kill" NARROW []
synonym: "lode" NARROW []
synonym: "moat" RELATED []
synonym: "narrows" NARROW []
synonym: "narrows" RELATED []
synonym: "narrows (hydrographic)" RELATED []
synonym: "overflow channel" NARROW []
synonym: "passage" NARROW []
synonym: "pup" NARROW []
synonym: "race" NARROW []
synonym: "ravine" NARROW []
synonym: "reach" NARROW []
synonym: "rill" NARROW []
synonym: "rivulet" NARROW []
synonym: "run" NARROW []
synonym: "runnel" NARROW []
synonym: "seachannel" NARROW []
synonym: "seaway" NARROW []
synonym: "spillway" NARROW []
synonym: "stream" NARROW []
synonym: "tideway" NARROW []
synonym: "wash" NARROW []
synonym: "water gap" NARROW []
is_a: ENVO:01000618 ! lotic water body

[Term]
id: ENVO:00000062
name: populated place
def: "Place or area with clustered or scattered buildings and a permanent human population." []
synonym: "inhabited place" EXACT []
synonym: "inhabited region" RELATED []
synonym: "place" BROAD []
synonym: "populated locality" RELATED []
synonym: "populated place" EXACT []
synonym: "populated places" EXACT []
synonym: "settlement" EXACT []
is_a: ENVO:00000070 ! constructed feature

[Term]
id: ENVO:00000063
name: water body
def: "An accumulation of water of varying size." []
synonym: "aquatic feature" EXACT []
synonym: "bodies of water" EXACT []
synonym: "body of water" EXACT []
synonym: "hydrographic feature" BROAD []
synonym: "waterbody" EXACT []
is_a: ENVO:00000000 ! geographic feature

[Term]
id: ENVO:00000070
name: constructed feature
def: "A feature that has been constructed by deliberate human effort." []
is_a: ENVO:00000002 ! anthropogenic geographic feature

[Term]
id: ENVO:00000123
name: political entity
def: "A geographical region whose affairs and population are administered by an authority." []
synonym: "political entity" RELATED []
is_a: ENVO:00000004 ! administrative region

[Term]
id: ENVO:00000124
name: supranational geopolitical entity
def: "A political entitity established by more than one state and with at least some influence over the affairs of its member states." []
is_a: ENVO:00000123 ! political entity

[Term]
id: ENVO:00000358
name: protected area
def: "An area of land and/or a body of water especially dedicated to the protection and maintenance of biological diversity, and of natural and associated cultural resources, and managed through legal or other effective means." []
is_a: ENVO:00000562 ! park

[Term]
id: ENVO:00000428
name: biome
def: "A biome is an environmental system to which resident ecological communities have evolved adaptations." []
synonym: "ecosystem" RELATED []
synonym: "EcosytemType" RELATED []
synonym: "major habitat type" EXACT []
is_a: ENVO:01000254 ! environmental system

[Term]
id: ENVO:00000446
name: terrestrial biome
def: "A biome that applies to the terrestrial realm." []
synonym: "terrestrial realm" RELATED []
is_a: ENVO:00000428 ! biome

[Term]
id: ENVO:00000559
name: weapons test site
def: "A region at which weapons, typically military, are tested." []
is_a: ENVO:00000002 ! anthropogenic geographic feature

[Term]
id: ENVO:00000560
name: nuclear weapons test site
def: "A weapons test site at which nuclear weapons are, or have been, tested." []
is_a: ENVO:00000559 ! weapons test site

[Term]
id: ENVO:00000562
name: park
def: "A bounded area of land, or water, usually in its natural or semi-natural (landscaped) state and set aside for some purpose, usually to do with recreation or conservation." []
is_a: ENVO:00000002 ! anthropogenic geographic feature

[Term]
id: ENVO:00000856
name: city
def: "Incorporated populated place." []
synonym: "urban area" BROAD []
is_a: ENVO:01000658 ! dense settlement

[Term]
id: ENVO:00001999
name: marine water body
def: "A significant accumulation of water which is part of a marine biome." []
synonym: "body of marine water" EXACT []
synonym: "marine waterbody" EXACT []
is_a: ENVO:01000617 ! lentic water body

[Term]
id: ENVO:00002001
name: waste water
def: "Water that has been adversely affected in quality by anthropogenic influence." []
is_a: ENVO:00002186 ! contaminated water
is_a: ENVO:00002264 ! waste material

[Term]
id: ENVO:00002006
name: water
def: "An environmental material primarily composed of dihydrogen oxide in its liquid form." []
is_a: ENVO:01000815 ! liquid environmental material

[Term]
id: ENVO:00002011
name: fresh water
synonym: "freshwater" EXACT []
is_a: ENVO:00002006 ! water

[Term]
id: ENVO:00002018
name: sewage
def: "Wastewater that is contaminated with feces or urine," []
is_a: ENVO:00002001 ! waste water

[Term]
id: ENVO:00002186
name: contaminated water
synonym: "polluted water" EXACT []
is_a: ENVO:00002006 ! water

[Term]
id: ENVO:00002193
name: pulp-bleaching waste water
is_a: ENVO:00002001 ! waste water

[Term]
id: ENVO:00002264
name: waste material
def: "A material which is not the desired output of a process and which is typically the input of a process which removes it from its producer (e.g. a disposal process)." []
is_a: ENVO:00010483 ! environmental material

[Term]
id: ENVO:00002297
name: environmental feature
def: "A material entity which determines an environmental system." []
is_a: BFO:0000040 ! material entity

[Term]
id: ENVO:00003064
name: drinking water
def: "Drinking water is water which may be consumed by humans with no adverse effects on their health." []
synonym: "potable water" EXACT []
is_a: ENVO:00002011 ! fresh water

[Term]
id: ENVO:00010483
name: environmental material
def: "A portion of environmental material is a fiat object which forms the medium or part of the medium of an environmental system." []
synonym: "portion of environmental material" EXACT []
is_a: BFO:0000040 ! material entity

[Term]
id: ENVO:01000219
name: anthropogenic terrestrial biome
def: "An anthropogenic terrestrial biome is a terrestrial biome which has community structures determined by human activity." []
synonym: "anthrome" EXACT []
synonym: "human biome" EXACT []
is_a: ENVO:00000446 ! terrestrial biome

[Term]
id: ENVO:01000245
name: cropland biome
def: "A cropland biome is an anthropogenic terrestrial biome which is primarily used for agricultural activity and which contains no village or larger human settlement." []
is_a: ENVO:01000219 ! anthropogenic terrestrial biome

[Term]
id: ENVO:01000246
name: village biome
def: "A village biome is an anthropogenic terrestrial biome which contains settlements such as villages, towns, and/or small cities and which is primarily used for agricultural activity." []
is_a: ENVO:01000219 ! anthropogenic terrestrial biome

[Term]
id: ENVO:01000247
name: rangeland biome
def: "A rangeland biome is an anthropogenic terrestrial biome which is primarily used for the rearing and grazing of livestock." []
is_a: ENVO:01000219 ! anthropogenic terrestrial biome

[Term]
id: ENVO:01000248
name: dense settlement biome
def: "A dense settlement biome is an anthropogenic terrestrial biome which is primarily used for human habitation, recreation, and industry within built structures with little other land use." []
is_a: ENVO:01000219 ! anthropogenic terrestrial biome

[Term]
id: ENVO:01000249
name: urban biome
def: "An urban biome is a dense settlement biome which has been urbanised." []
is_a: ENVO:01000248 ! dense settlement biome

[Term]
id: ENVO:01000254
name: environmental system
def: "A system which has the disposition to environ one or more material entities." []
synonym: "environment" EXACT []
is_a: RO:0002577 ! system

[Term]
id: ENVO:01000266
name: water vapour
def: "Water vapour is a vapour which is the gas phase of water." []
synonym: "aqueous vapor" EXACT []
synonym: "aqueous vapour" EXACT []
synonym: "water vapor" EXACT []
is_a: ENVO:01000797 ! gaseous environmental material

[Term]
id: ENVO:01000268
name: atmospheric water vapour
def: "Atmospheric water vapour is water vapour that is part of an atmosphere." []
synonym: "atmospheric water vapor" EXACT []
is_a: ENVO:01000266 ! water vapour

[Term]
id: ENVO:01000408
name: environmental zone
def: "An environmental zone is an environmental feature whose extent is determined by the presence or influence of one or more material entities or processes. An environmental zone may, itself, assume the role of an environmental feature." []
synonym: "environmental area" RELATED []
is_a: ENVO:00002297 ! environmental feature

[Term]
id: ENVO:01000451
name: atmospheric carbon dioxide
def: "Atmospheric carbon dioxide is an environmental material composed of carbon dioxide in its gaseous form present in the atmosphere." []
is_a: ENVO:01000797 ! gaseous environmental material

[Term]
id: ENVO:01000537
name: atmospheric ozone
def: "Atmospheric ozone is an environmental material primarily composed of ozone in its gaseous form and present in the atmosphere." []
synonym: "atmospheric ozone" RELATED []
is_a: ENVO:01000797 ! gaseous environmental material

[Term]
id: ENVO:01000617
name: lentic water body
def: "A lentic water body is a water body in which the accumulated water, in its totality, has very little to no directed flow." []
is_a: ENVO:00000063 ! water body

[Term]
id: ENVO:01000618
name: lotic water body
def: "A lotic water body is a water body in which the accumulated water, in its totality, is flowing." []
is_a: ENVO:00000063 ! water body

[Term]
id: ENVO:01000629
name: climate change
def: "The long-term fluctuations in temperature, precipitation, wind, and all other aspects of the Earth's climate. External processes, such as solar-irradiance variations, variations of the Earth's orbital parameters (eccentricity, precession, and inclination), lithosphere motions, and volcanic activity, are factors in climatic variation. Internal variations of the climate system, e.g., changes in the abundance of greenhouse gases, also may produce fluctuations of sufficient magnitude and variability to explain observed climate change through the feedback processes interrelating the components of the climate system." []
is_a: ENVO:02500000 ! environmental system process

[Term]
id: ENVO:01000634
name: volcanic eruption
def: "A volcanic process is a process during which lava, tephra (ash, lapilli, volcanic bombs and blocks), and assorted gases are expelled from a volcanic vent or fissure." []
is_a: ENVO:02500031 ! hydrological process

[Term]
id: ENVO:01000653
name: slum
def: "A slum is a heavily populated urban informal settlement with substandard housing in which households lack any one of the following: access to improved water, access to improved sanitation, sufficient-living area, durability of housing, or security of tenure." []
is_a: ENVO:01000658 ! dense settlement

[Term]
id: ENVO:01000655
name: explosive eruption
def: "An explosive eruption is a volcanic process in which pressurised magma is violently expelled and froths into volcanic ash. Explosive eruptions can eject a cloud of rocks, dust, gas, and pyroclastic material  which may then collapse, creating a pyroclastic flow of hot volcanic matter." []
is_a: ENVO:01000634 ! volcanic eruption

[Term]
id: ENVO:01000656
name: effusive eruption
def: "An effusive eruption is a volcanic eruption during which lava flows onto the ground." []
is_a: ENVO:01000634 ! volcanic eruption

[Term]
id: ENVO:01000658
name: dense settlement
def: "A settlement with a high density of buildings and inhabitants." []
is_a: ENVO:00000062 ! populated place

[Term]
id: ENVO:01000665
name: waste role
def: "A role that is realized in some process wherein the bearer is discarded or not utilized further." []
is_a: BFO:0000023 ! role

[Term]
id: ENVO:01000677
name: earthquake
def: "An earthquake is a process whereby part of the surface of a planet shakes due to the passage of seismic waves through rocks. Seismic waves are produced when some form of energy stored in a planet's crust is suddenly released. Elastic strain, gravity, chemical reactions, or even the motion of massive bodies can produce earthquakes." []
is_a: ENVO:02500000 ! environmental system process

[Term]
id: ENVO:01000678
name: tectonic earthquake
def: "A tectonic earthquake is an earthquake caused by the release of elastic strain. A tectonic earthquake occurs when strains in rock masses have accumulated to a point where the resulting stresses exceed the strength of the rocks, and sudden fracturing results." []
is_a: ENVO:01000677 ! earthquake

[Term]
id: ENVO:01000679
name: megathrust earthquake
def: "A megathrust earthquake is a tectonic earthquake which occurs at subduction zones at destructive plate boundaries (convergent boundaries). These interplate earthquakes are the planet's most powerful, with moment magnitudes that can exceed 9.0." []
is_a: ENVO:01000678 ! tectonic earthquake

[Term]
id: ENVO:01000680
name: polluted lake
def: "A lake which has concentrations of environmental contaminants high enough to harm the ecosystems associated with it." []
is_a: ENVO:00000020 ! lake

[Term]
id: ENVO:01000687
name: coast
def: "A coast is the area where land meets the sea, ocean, or lake." []
is_a: ENVO:00000000 ! geographic feature

[Term]
id: ENVO:01000689
name: tsunami
def: "A tsunami is a process during which a series of waves is generated in a water body, typically an ocean or large lake, by the displacement of a large volume of water. Earthquakes, volcanic eruptions and other underwater explosions (including detonations of underwater nuclear devices), landslides, glacier calvings, meteorite impacts and other disturbances above or below water all have the potential to generate a tsunami." []
synonym: "seismic sea wave" EXACT []
synonym: "tidal wave" EXACT []
is_a: ENVO:02500000 ! environmental system process

[Term]
id: ENVO:01000690
name: mass wasting
def: "Mass wasting is the geomorphic process by which solid environmental material such as soil, sand, regolith, and/or rock move downslope typically as a mass, largely under the force of gravity, but frequently affected by water and water content as in submarine environments and mudslides." []
synonym: "mass movement" BROAD []
synonym: "slope movement" EXACT []
is_a: ENVO:03000010 ! material transport process

[Term]
id: ENVO:01000691
name: avalanche
def: "An avalanche is a rapid flow of snow down a sloping surface." []
synonym: "snowslide" EXACT []
synonym: "snowslip" EXACT []
is_a: ENVO:01000696 ! mass wasting flow

[Term]
id: ENVO:01000692
name: landslide process
def: "A landslide is a process whereby a large mass of earth and rocks moves down a hill or a mountainside." []
synonym: "landslip" EXACT []
is_a: ENVO:01000690 ! mass wasting

[Term]
id: ENVO:01000693
name: rockfall
is_a: ENVO:01000690 ! mass wasting

[Term]
id: ENVO:01000694
name: geological subsidence
def: "A subsidence process is a geomorphologic process in which a surface shifts downward relative to a datum such as sea-level." []
synonym: "subsidence" BROAD []
is_a: ENVO:03000010 ! material transport process

[Term]
id: ENVO:01000695
name: mudslide
is_a: ENVO:01000690 ! mass wasting

[Term]
id: ENVO:01000696
name: mass wasting flow
def: "A mass wasting flow is a form of mass wasting during which the moving materials behave similarly to a flowing fluid. Water, air and ice are often involved in enabling fluidlike motion of the material." []
synonym: "flow" BROAD []
is_a: ENVO:01000690 ! mass wasting

[Term]
id: ENVO:01000697
name: mudflow
def: "A mudflow is a form of mass wasting which involves very rapid to extremely rapid surging flow of debris that has become partially or fully liquified by the addition of significant amounts of water to clay-rich source material." []
synonym: "mud flow" EXACT []
is_a: ENVO:01000696 ! mass wasting flow

[Term]
id: ENVO:01000698
name: debris flow
is_a: ENVO:01000696 ! mass wasting flow

[Term]
id: ENVO:01000699
name: lahar
def: "A lahar is a type of mudflow or debris flow composed of a slurry of pyroclastic material, rocky debris, and water. The material flows down from a volcano, typically along a river valley." []
is_a: ENVO:01000697 ! mudflow

[Term]
id: ENVO:01000700
name: sturzstrom
def: "A sturzstrom is a landslide consisting which has a great amount of kinetic energy resulting in greater horizontal movement when compared to its initial vertical drop â€” as much as 20 or 30 times the vertical distance. By contrast a normal landslide will typically travel a horizontal distance that is less than twice the distance that the material has fallen." []
is_a: ENVO:01000692 ! landslide process

[Term]
id: ENVO:01000702
name: ash fall process
def: "An ash fall process is a process in which volcanic ash formed during an explosive volcanic eruption, phreatomagmatic eruption, or during material transport in pyroclastic density currents is pulled towards the planetary surface by gravity." []
is_a: ENVO:01000875 ! precipitation process

[Term]
id: ENVO:01000707
name: coastal flooding
def: "Coastal flooding is a process in which normally dry, low-lying land near a coast is flooded by sea water." []
is_a: ENVO:02500002 ! flooding

[Term]
id: ENVO:01000708
name: riverine flooding
def: "Riverine flooding is a process in which the flow rate of river water exceeds the capacity of its channel, thus flooding neighbouring land. Bends and meanders in a river channel are particularly disposed to such flooding." []
is_a: ENVO:02500002 ! flooding

[Term]
id: ENVO:01000709
name: flash flooding
def: "Flash flooding is a process in which low-lying land is inundated with water for a short period of time and are usually the result of precipitation or a breach in the container of a water body." []
is_a: ENVO:02500002 ! flooding

[Term]
id: ENVO:01000710
name: flood
def: "An unusual accumulation of water above the ground caused by high tide, heavy rain, melting snow or rapid runoff from paved areas." []
is_a: ENVO:00000063 ! water body

[Term]
id: ENVO:01000711
name: coastal flood
def: "A coastal flood is a flood which is formed as a result of large amounts of water from marine water bodies or large lakes being transported to usually dry land by displacement processes such as high winds or seismic activity." []
is_a: ENVO:01000710 ! flood

[Term]
id: ENVO:01000712
name: riverine flood
def: "A riverine flood is a flood which is formed as a result of a river's flow rate exceeding the capacity of its channel." []
is_a: ENVO:01000710 ! flood

[Term]
id: ENVO:01000713
name: flash flood
def: "A flash flood is a flood formed by the rapid flooding of geomorphic low-lying areas. It may be caused by heavy rain associated with a severe thunderstorm, hurricane, tropical storm, or meltwater from ice or snow flowing over ice sheets or snowfields. Flash floods may also occur after the collapse of a natural ice or debris dam, or a human structure such as a man-made dam. Flash floods are distinguished from a regular flood by a timescale of less than six hours." []
is_a: ENVO:01000710 ! flood

[Term]
id: ENVO:01000714
name: storm surge
def: "A storm surge is a coastal flood which is caused by low-pressure weather systems such as tropical cyclones and strong extratropical cyclones, the severity of which is affected by the shallowness and orientation of the water body relative to storm path, and the timing of tides." []
is_a: ENVO:01000711 ! coastal flood

[Term]
id: ENVO:01000715
name: metotsunami
def: "A meteotsunami is a tsunami caused by atmospheric processes and differences in air pressure." []
is_a: ENVO:01000689 ! tsunami

[Term]
id: ENVO:01000716
name: storm surge process
def: "A storm surge process is a coastal flooding process which is caused by low pressure weather systems such as tropical cyclones and strong extratropical cyclones, the severity of which is affected by the shallowness and orientation of the water body relative to storm path, and the timing of tides." []
is_a: ENVO:01000707 ! coastal flooding

[Term]
id: ENVO:01000717
name: areal flooding
def: "Areal flooding is a flooding process in which flat or low-lying areas become inundated with water due to water input exceeding infiltration, evaporation, or run off." []
is_a: ENVO:02500002 ! flooding

[Term]
id: ENVO:01000718
name: urban flooding
def: "Urban flooding is a flooding process in which land or property in a built environment, particularly in more densely populated areas, is inundated due to the rate of water input exceeding that of water drainage provided by the environment's drainage systems." []
is_a: ENVO:02500002 ! flooding

[Term]
id: ENVO:01000730
name: lava flow process
def: "A process in which a volume of lava emitted during an effusive eruption moves along a solid surface." []
is_a: ENVO:02500000 ! environmental system process

[Term]
id: ENVO:01000741
name: recycling process
def: "A process in which some input bearing a waste role is consumed to produce an output which bears a resource role." []
is_a: ENVO:02500000 ! environmental system process

[Term]
id: ENVO:01000742
name: carbon-bearing gas emission process
def: "A carbon emission process is any environmental process which outputs a carbon-bearing gas." []
synonym: "carbon emission process" BROAD []
is_a: ENVO:03000093 ! hydrocarbon gas emission process

[Term]
id: ENVO:01000743
name: land consumption process
def: "A process in which natural ecosystems present over an expanse of land are removed and replaced with anthropogenic ecosystems." []
is_a: ENVO:02500005 ! land degradation

[Term]
id: ENVO:01000744
name: human dwelling
def: "A self-contained constructed feature used by one or more households as a home, such as a house, apartment, mobile home, houseboat or other 'substantial' structure. A dwelling typically includes nearby outbuildings, sheds etc. within the curtilage of the property, excluding any 'open fields beyond'. It has significance in relation to search and seizure, conveyancing of real property, burglary, trespass, and land use planning." []
is_a: ENVO:00000070 ! constructed feature

[Term]
id: ENVO:01000762
name: sparsely populated settlement
def: "A settlement with a low density of buildings and inhabitants." []
is_a: ENVO:00000062 ! populated place

[Term]
id: ENVO:01000763
name: rural settlement
def: "A settlement which has lower population density than a town, city, or other urban environment and is primarily used for agricultural or pastoral activity." []
is_a: ENVO:01000762 ! sparsely populated settlement

[Term]
id: ENVO:01000764
name: formal settlement
def: "A settlement which has been established and is managed through officially sanctioned processes and is recognised as legal by a competent authority." []
is_a: ENVO:00000062 ! populated place

[Term]
id: ENVO:01000765
name: informal settlement
def: "A settlement which is not associated with or directed by official planning processes and which typically lacks municipal services and infrastructure such as sanitation, water services, and waste management services." []
is_a: ENVO:00000062 ! populated place

[Term]
id: ENVO:01000767
name: illegal settlement
def: "A settlement on land that the inhabitants have no legal claim to or occupy illegally." []
is_a: ENVO:00000062 ! populated place

[Term]
id: ENVO:01000769
name: carbon dioxide emission process
def: "A carbon emission process is any environmental process which releases carbon dioxide gas into the atmosphere." []
is_a: ENVO:01000742 ! carbon-bearing gas emission process

[Term]
id: ENVO:01000770
name: carbon dioxide emission
def: "A volume of carbon dioxide gas emitted by a carbon dioxide emission process." []
is_a: ENVO:01000797 ! gaseous environmental material

[Term]
id: ENVO:01000772
name: rural area
def: "An area which is outside of a town, city, or urban area. Rural areas are primarily used for agriculture or pastoralism and may contain rural settlements." []
is_a: ENVO:01000408 ! environmental zone

[Term]
id: ENVO:01000773
name: village
def: "A village is a clustered human settlement or community, larger than a hamlet but smaller than a town, with a population ranging from a few hundred to a few thousand. Though often located in rural areas, the term urban village is also applied to certain urban neighbourhoods. Villages are normally permanent, with fixed dwellings; however, transient villages can occur. Further, the dwellings of a village are fairly close to one another, not scattered broadly over the landscape, as a dispersed settlement." []
is_a: ENVO:00000062 ! populated place

[Term]
id: ENVO:01000778
name: important site
def: "An environmental zone which contains, as determined by an officially mandated selection process, one or more ecosystems which include, as parts, ecological communities of global significance for conservation due to their vulnerability and irreplaceability." []
synonym: "Alliance for Zero Extinction Sites" NARROW []
synonym: "Ecologically and Biologically Significant Area" NARROW []
synonym: "Important Bird Area" NARROW []
synonym: "Important Mammal Area" NARROW []
synonym: "Important Plant Area" NARROW []
synonym: "Important Site for Freshwater Biodiversity" NARROW []
synonym: "IUCN Important Site for Freshwater Biodiversity" NARROW []
synonym: "key biodiversity area" EXACT []
synonym: "Prime Butterfly Area" NARROW []
synonym: "Ramsar Sites" NARROW []
is_a: ENVO:01000408 ! environmental zone

[Term]
id: ENVO:01000779
name: public infrastructure
def: "The system of public works in a country, state or region, including roads, utility lines and public buildings." []
synonym: "infrastructure" BROAD []
is_a: ENVO:00000070 ! constructed feature

[Term]
id: ENVO:01000784
name: illegal informal settlement
def: "A populated place where groups of housing units have been constructed on land that the occupants have no legal claim to, or occupy illegally, or where dwellings are not in compliance with current planning and building regulations." []
synonym: "informal settlement" BROAD []
is_a: ENVO:01000765 ! informal settlement

[Term]
id: ENVO:01000785
name: material extraction process
def: "A planned process during which a portion of environmental material is removed from a material entity." []
is_a: ENVO:02500000 ! environmental system process

[Term]
id: ENVO:01000797
name: gaseous environmental material
def: "A material entity which is composed of one or more chemical entities and has neither independent shape nor volume but tends to expand indefinitely." []
synonym: "gas" NARROW []
is_a: ENVO:00010483 ! environmental material

[Term]
id: ENVO:01000815
name: liquid environmental material
def: "An environmental material which is in a liquid state." []
is_a: ENVO:00010483 ! environmental material

[Term]
id: ENVO:01000875
name: precipitation process
def: "A precipitation process is a process in which a portion of some substance segregates from a material in which that substance or its precursors were dissolved or suspended in and settles due to a force such as gravity or centrifugal force." []
is_a: ENVO:03000010 ! material transport process

[Term]
id: ENVO:01000930
name: ecological corridor
def: "An ecosystem which bridges two or more adjoing ecosystems and through which organisms may move or propagate." []
synonym: "animal corridor" RELATED []
synonym: "green corridor" RELATED []
synonym: "habitat corridor" RELATED []
synonym: "wildlife corridor" RELATED []
is_a: ENVO:01000254 ! environmental system

[Term]
id: ENVO:02500000
name: environmental system process
is_a: BFO:0000015 ! process

[Term]
id: ENVO:02500001
name: desertification
def: "a type of land degradation in which a relatively dry land region becomes increasingly arid, typically losing its bodies of water as well as vegetation and wildlife." []
is_a: ENVO:02500000 ! environmental system process

[Term]
id: ENVO:02500002
name: flooding
def: "A general and temporary condition of partial or complete inundation of normally dry land areas from the overflow of inland and/or tidal waters, and/or the unusual and rapid accumulation or runoff of surface waters from any source. A great flow along a watercourse or a flow causing inundation of lands not normally covered by water." []
is_a: ENVO:02500000 ! environmental system process

[Term]
id: ENVO:02500005
name: land degradation
def: "A process which diminishes the functioning of an ecosystem located on land." []
is_a: ENVO:02500000 ! environmental system process

[Term]
id: ENVO:02500011
name: afforestation
def: "Establishment of a new forest by seeding or planting of nonforested land." []
is_a: ENVO:02500000 ! environmental system process

[Term]
id: ENVO:02500012
name: deforestation
def: "The removal of forest and undergrowth to, for example, increase the surface of arable land or to use the timber for construction or industrial purposes." []
synonym: "clearance" BROAD []
synonym: "clearing" BROAD []
is_a: ENVO:02500000 ! environmental system process

[Term]
id: ENVO:02500013
name: reforestation
def: "The planting of trees in areas in where forests have previously been cleared." []
is_a: ENVO:02500032 ! revegetation

[Term]
id: ENVO:02500017
name: anthropogenic reforestation
is_a: ENVO:02500013 ! reforestation
is_a: ENVO:02500027 ! anthropogenic environmental process

[Term]
id: ENVO:02500026
name: anthropogenic modulatory intervention process
is_a: ENVO:02500027 ! anthropogenic environmental process

[Term]
id: ENVO:02500027
name: anthropogenic environmental process
is_a: ENVO:02500000 ! environmental system process

[Term]
id: ENVO:02500031
name: hydrological process
is_a: ENVO:02500000 ! environmental system process

[Term]
id: ENVO:02500032
name: revegetation
is_a: ENVO:02500000 ! environmental system process

[Term]
id: ENVO:02500036
name: environmental pollution
def: "An environmental system process that results in the introduction of contaminants into an environment." []
synonym: "pollution" EXACT []
is_a: ENVO:02500000 ! environmental system process

[Term]
id: ENVO:02500037
name: air pollution
def: "A pollution process that releases particulates into the atmosphere." []
is_a: ENVO:02500036 ! environmental pollution

[Term]
id: ENVO:02500038
name: soil pollution
def: "A pollution process during which soil is contaminated." []
is_a: ENVO:02500036 ! environmental pollution

[Term]
id: ENVO:02500039
name: water pollution
def: "A pollution process during which water is contaminated." []
is_a: ENVO:02500036 ! environmental pollution

[Term]
id: ENVO:02500040
name: plastic pollution
def: "A pollution process that results in increased levels of plastic in the environment." []
is_a: ENVO:02500036 ! environmental pollution

[Term]
id: ENVO:02500041
name: environmental monitoring
def: "An process in which environmental parameters and variables are continually assayed." []
synonym: "monitoring" BROAD []
is_a: ENVO:02500000 ! environmental system process

[Term]
id: ENVO:02500042
name: pollution control
synonym: "pollution prevention" NARROW []
is_a: ENVO:02500026 ! anthropogenic modulatory intervention process

[Term]
id: ENVO:02500043
name: pollution monitoring
def: "A monitoring process that assays the level of environmental pollutants to determine the presence of effect of environmental pollution." []
is_a: ENVO:02500041 ! environmental monitoring

[Term]
id: ENVO:02500044
name: urban pollution
def: "A pollution process that results in increased levels of pollutants in an urban environment." []
is_a: ENVO:02500036 ! environmental pollution

[Term]
id: ENVO:03000010
name: material transport process
def: "A process during which material is displaced from it's original location and transported either to a new location or back to the original location." []
is_a: ENVO:02500000 ! environmental system process

[Term]
id: ENVO:03000092
name: gas emission process
def: "A material transport process during which a portion of gaseous environmental material is transported into the atmosphere." []
is_a: ENVO:03000010 ! material transport process

[Term]
id: ENVO:03000093
name: hydrocarbon gas emission process
def: "A gas emission process during which a portion of hydrocarbon gas is transported into the atmosphere." []
is_a: ENVO:03000092 ! gas emission process

[Term]
id: RO:0002577
name: system
def: "A material entity consisting of multiple components that are causally integrated." []
is_a: BFO:0000040 ! material entity

