format-version: 1.2
ontology: http://purl.unep.org/sdg/imports/pco_import.owl

[Term]
id: PCO:0000000
name: collection of organisms
def: "A material entity that consists of two or more organisms, viruses, or viroids." []

[Term]
id: PCO:0000001
name: population
def: "A collection of organisms, all of the same species, that live in the same place." []
is_a: PCO:0000018 ! collection of organisms of the same species

[Term]
id: PCO:0000002
name: ecological community
def: "A collection of organisms of at least two different species, living in a particular area." []
is_a: PCO:0000000 ! collection of organisms

[Term]
id: PCO:0000018
name: collection of organisms of the same species
def: "A material entity that has as parts two or more organisms, viruses, or viroids of the same species and no members of any other species." []
is_a: PCO:0000000 ! collection of organisms

